Commit for submission

src/fol.lean
@@ -9,20 +9,20 @@ proof calculus.
 
 ## Main result
 
-- `formula 𝒮` : the definition of first-order formulas over a signature 𝒮
-- `proof 𝒮`   : the definition of proof terms of natural deduction over a signature 𝒮
+- `formula σ`      : the definition of first-order formulas over a signature σ
+- `proof_term σ`   : the definition of proof terms of natural deduction over a signature σ
 
 ## Notations
 
 We define the following notations for lifts and substitutions:
 
-- `X ↑ m ＠ i` for `lift X s k`  where `X` can be a term, a formula or a set of formulas.
-- `X[ s ⁄ k ]` for `subst X s k` where `X` can be a term, a formula or a set of formulas.
-- `Γ ⊢ φ` for proof Γ φ  
+- `X ↑ m ＠ i` for `lift X s k`  where `X` can be a term or a formula .
+- `X[ s ⁄ k ]` for `subst X s k` where `X` can be a term or a formula .
+- `Γ ⊢ φ` for `proof_term Γ φ` 
 
 We use the following local notations
 
-- `::` for `set.insert`
+- `>>` for `set.insert`
 
 ## Notes
 
@@ -32,12 +32,14 @@ This includes some definitions that are not part of the actual implementation bu
 ## References
 
 * [N.G. de Bruijn, *Lambda calculus notation with nameless dummies*] [DB72]
-  -- the original paper describing what is now called de Bruijn indices
-* [J.M. Han, F.van Doorn, *A Formal Proof of the Independence of the Continuum Hypothesis*] [HvD20]
-  -- which we followed in their implementation of first-order logic using "partially applied" terms and formulas 
+  -- the original paper describing de Bruijn indices
+* [J.M. Han, F.van Doorn, *A Formal Proof of the Independence of the Continuum Hypothesis*] [HD20]
+  -- we followed their implementation of first-order logic using "partially applied" terms and formulas 
   -- See also: https://flypitch.github.io/
-* [M.Huth, M. Ryan, *Logic in computer science*] [HR04]
-  -- for their development of the natural deduction proof calculus
+* [I. Chiswell, W. Hodges,*Mathematical Logic*] [CH04]
+  -- first order logic and natural deduction
+* [M. Huth, M. Ryan, *Logic in computer science*] [HR04]
+  -- first order logic and natural deduction
 * [S. Berghofer, C. Urban, *A Head-to-Head Comparison of de Bruijn Indices and Names*] [BH07]
   -- for a good breakdown of the proof of the substitution lemma `subst_subst`
 * https://github.com/coq-community/dblib/blob/master/src/DeBruijn.v 
@@ -46,132 +48,77 @@ This includes some definitions that are not part of the actual implementation bu
 
 -- use with `simp only with tls`
 mk_simp_attribute tls
-"Collection of definitions and lemmas for simplifying combinations of lifts and substitutions we would consider trivial."
+"Collection of definitions and lemmas for simplifying trivial  combinations of lifts and substitutions."
 
 open nat set
-namespace fol
 universe variable u
 
+namespace fol
 /-- A signature of a first-order logic defining its function and predicate symbols with arities. -/
 structure signature : Type (u+1) :=
 (func_symb : ℕ → Type u) (pred_symb : ℕ → Type u)
 
-def signature.constants (𝒮 : signature) := 𝒮.func_symb 0
+def signature.constants (σ : signature) := σ.func_symb 0
 
 inductive sorry_nothing : ℕ → Type u
 
 def trivial_signature : signature :=
 { func_symb := sorry_nothing, pred_symb := sorry_nothing}
 
+variable (σ : signature.{u})
 
 /-! ### terms -/
-variable (𝒮 : signature.{u})
-
 /--
-  `preterm 𝒮 a` is partially applied term of first-order logic over the signature `𝒮`.
+  `preterm σ a` is partially applied term of first-order logic over the signature `σ`.
   If applied to `a` terms it becomes a well-formed term.
 -/
 inductive preterm : ℕ → Type u
 | var  (index : ℕ) : preterm 0
-| func {arity : ℕ} (f : 𝒮.func_symb arity) : preterm arity
+| func {arity : ℕ} (f : σ.func_symb arity) : preterm arity
 | fapp {arity : ℕ} (t : preterm (arity+1))  (s : preterm 0) : preterm arity
 
 export preterm
 
 prefix `#`:max := preterm.var
-@[reducible] def term := preterm 𝒮 0
+@[reducible] def term := preterm σ 0
 
-variable {𝒮}
-
-/-  
-  ## Definition - variables at `k`  
-  
-  Let `t` be a term. The variables of `t` are defined by structural induction in the obvious way.
-
-  Let `k ∈ ℕ`. The variables of `t` *at reference depth `k`* or simply *at `k`* are the variables 
-  of `t` such that their index is equal to `k`. 
-
-  A variable of `t` is called *`k`-free* if its index is greater than `k`.
-
-  The term `t` is called *`k`-free* if it all its variables are `k`-free.
-
-  ## Remark
-  The terminology of "reference depth" comes from de Bruijn's original paper. 
-  What do these variable indices reference? 
-  In the case of terms is easy to explain.
-  One should first imagine an sequence (called the environment) 
-      `...,x₃,x₂,x₁,x₀`
-  of what we will call "variable binders".
-
-  Variables at reference depth `k` then should be thought of referencing `xₖ`,
-  or, our preferred terminology, `xₖ` binds the variables at `k`.
-  The reason for writing this sequence from left to right will hopefully become apparent 
-  when we introduce formulas.
-
-  We will sometimes refer to variable binders as variables of the environment or simply variable
-  if it does not cause confusion.
--/
-
+variable {σ}
 
 namespace term
 
-/-
-  Even though we technically have an infinite amount of variables
-  it is often very convenient to be able to add "fresh" variables
-  to the environment. In the most common case one adds a single new
-  variable right at the start of our imagined environment:
-    `...,x₃,x₂,x₁,x₀` to `...,x₃,x₂,x₁,x₀,y`. 
-  If we want the variables of `t` to reference the same variable binder
-  we will need to increase all indices by `1`. 
-  Doing so also ensures that the variable binder `y` is truly 
-  "fresh" for `t` in the sense that no variable of `t` is bound by it.
-
-  The case for adding `m` fresh variables at index `i` to the environment 
-  follows similarly.
-  It describes the change from
-    `...xᵢ₊₁,xᵢ,xᵢ₋₁,...,x₃,x₂,x₁,x₀`
-  to the new environment 
-    `....xᵢ₊₁,xᵢ,yₘ₋₁,...,y₀,xᵢ₋₁,...,x₃,x₂,x₁,x₀`.
-  We ensure consistent variable bindings of a term `t` by adding 
-  `m` to each `i`-free variable of `t`.
-
-  This operation on terms is know as a lift (or sometimes shift).
--/
-
-/--
-  `lift t m i` increases the index of each `i`-free variable in `t` by `m`.
--/
-def lift : ∀{a} , preterm 𝒮 a → ℕ → ℕ → preterm 𝒮 a 
-| _ #x          m i := #( if i ≤ x then x+m else x)
+/-- `lift t m i` increases the index of each `i`-free variable in `t` by `m`. -/
+def lift : ∀{a} , preterm σ a → ℕ → ℕ → preterm σ a 
+| _ #x          m i := #(if i ≤ x then x+m else x)
 | _ (func f)    m i := func f
 | _ (fapp t s)   m i := fapp (lift t m i) (lift s m i)
 
 end term
 
+-- we use ＠ (U+FF20) instead of the regular @ (U+0040)
 notation t ` ↑ `:90 m ` ＠ `:90 i:90  := term.lift t m i
 
 namespace term
 
 -- unfolding lemmas for the simplifier
-@[simp, tls] lemma lift_fapp {a} (t : preterm 𝒮 (a+1)) (s : preterm 𝒮 0) (m i : ℕ) 
+@[simp, tls] lemma lift_fapp {a} (t : preterm σ (a+1)) (s : preterm σ 0) (m i : ℕ) 
   : (fapp t s) ↑ m ＠ i = fapp (t ↑ m ＠ i) (s ↑ m ＠ i) := by refl
-@[simp, tls] lemma lift_func {a} (f : 𝒮.func_symb a) (m i : ℕ ) 
+@[simp, tls] lemma lift_func {a} (f : σ.func_symb a) (m i : ℕ) 
   : (func f) ↑ m ＠ i = func f := by refl
 
 -- lifting of variables by cases for the simplifier
-@[simp] lemma lift_var_lt {x m i : ℕ} (H : x < i) : #x ↑ m ＠ i = (#x : term 𝒮) 
+@[simp] lemma lift_var_lt {x m i : ℕ} (H : x < i) : #x ↑ m ＠ i = (#x : term σ) 
   := begin unfold lift, rw if_neg (not_le.mpr H), end
-@[simp, tls] lemma lift_var_eq {x m}: ((#x ↑ m ＠ x) = (#(x+m) : term 𝒮)) 
+@[simp, tls] lemma lift_var_eq {x m}: ((#x ↑ m ＠ x) = (#(x+m) : term σ)) 
   := begin rw lift, rw if_pos x.le_refl, end
-@[simp] lemma lift_var_gt {x m i} (H : i < x ) : #x ↑ m ＠ i = (#(x+m) : term 𝒮)
+@[simp] lemma lift_var_gt {x m i} (H : i < x) : #x ↑ m ＠ i = (#(x+m) : term σ)
   := begin rw lift, rw if_pos (le_of_lt H), end
-@[simp] lemma lift_var_ge {x m i} (H : i ≤ x ) : #x ↑ m ＠ i = (#(x+m) : term 𝒮)
+@[simp] lemma lift_var_ge {x m i} (H : i ≤ x) : #x ↑ m ＠ i = (#(x+m) : term σ)
   := begin rw lift, rw if_pos H, end
-@[simp] lemma lift_var_nge {x m i : ℕ} (H : ¬ i ≤ x) : #x ↑ m ＠ i = (#x : term 𝒮) 
+@[simp] lemma lift_var_nge {x m i : ℕ} (H : ¬ i ≤ x) : #x ↑ m ＠ i = (#x : term σ) 
   := begin unfold lift, rw if_neg H, end
 
 
-@[simp, tls] lemma lift_by_0: ∀ {a} ( t : preterm 𝒮 a) {i}, t ↑ 0 ＠ i = t
+@[simp, tls] lemma lift_by_0: ∀ {a} (t : preterm σ a) {i}, t ↑ 0 ＠ i = t
 | _ #x         i  := by simp[lift]
 | _ (func f)   _  := by refl
 | _ (fapp f t) _  := begin unfold lift, congr; apply lift_by_0, end
@@ -179,7 +126,7 @@ namespace term
 
 /- Various lifting lemmas. -/
 
-lemma lift_lift: ∀ {a} ( t : preterm 𝒮 a ) (m) {i} (n) {j} (H : j ≤ i), 
+lemma lift_lift: ∀ {a} (t : preterm σ a) (m) {i} (n) {j} (H : j ≤ i), 
   (t ↑ m ＠ i) ↑ n ＠ j = (t ↑ n ＠ j) ↑ m ＠ (i+n) 
 | _ #x          m i n j H   := 
   begin by_cases h₀ : i ≤ x,
@@ -187,60 +134,42 @@ lemma lift_lift: ∀ {a} ( t : preterm 𝒮 a ) (m) {i} (n) {j} (H : j ≤ i),
       have h₂ : j ≤ x + m := le_trans h₁ (x.le_add_right m),
       simp[*, add_right_comm], },
     { have h₁ : ¬(i + n ≤  x + n) := begin intro h, exact  h₀ (le_of_add_le_add_right h) end,
-      have h₂ : ¬(i + n ≤ x)      := begin intro h, exact h₁ ( le_trans h (x.le_add_right n) ) end,
+      have h₂ : ¬(i + n ≤ x)      := begin intro h, exact h₁ (le_trans h (x.le_add_right n)) end,
       by_cases j ≤ x; simp[*], }, 
   end
 | _ (func f)    _ _ _ _ _      := by refl
 | _ (fapp f t)  _ _ _ _ _   := by simp*
     
-
-lemma lift_lift_reverse {a} ( t : preterm 𝒮 a ) {m i} (n) {j} (H : i + m ≤ j)
-    : (t ↑ m ＠ i) ↑ n ＠ j = ( t ↑ n ＠ (j-m) ) ↑  m  ＠ i :=
+lemma lift_lift_reverse {a} (t : preterm σ a) {m i} (n) {j} (H : i + m ≤ j) : 
+  (t ↑ m ＠ i) ↑ n ＠ j = (t ↑ n ＠ (j-m)) ↑ m ＠ i :=
 begin
   have h : i ≤ (j-m) := nat.le_sub_right_of_add_le H,
   have h': m ≤ j := (le_trans (m.le_add_left i) H),
   rw [lift_lift t n m h, nat.sub_add_cancel h'],
 end
 
-lemma lift_lift_merge: ∀ {a} ( t : preterm 𝒮 a) {m i} (n) {j} (H : i ≤ j) (H' : j ≤ i + m), 
-  (t ↑ m ＠ i ) ↑ n ＠ j = t ↑ (m+n) ＠ i
+lemma lift_lift_merge: ∀ {a} (t : preterm σ a) {m i} (n) {j} (H : i ≤ j) (H' : j ≤ i + m), 
+  (t ↑ m ＠ i) ↑ n ＠ j = t ↑ (m+n) ＠ i
 | _ #x         m i n j H H' :=  
   begin by_cases h₀ : i ≤ x,
     { have h₁ : j ≤ x + m  := le_trans H' (add_le_add_right h₀ m),
       simp[*, add_assoc], },
-    { have h₁ : ¬ ( j ≤ x) := (λ h,  h₀ (le_trans H h)),
+    { have h₁ : ¬ (j ≤ x) := (λ h,  h₀ (le_trans H h)),
       simp[*], }, 
   end
 | _ (func f)   _ _ _ _ _ _  := by refl
 | _ (fapp t s) _ _ _ _ _ _  := by simp*
 
-lemma lift_by_succ {a} ( t : preterm 𝒮 a) {m i} : t ↑ (m+1) ＠ i  = ( t ↑ 1 ＠ i) ↑ m ＠ i
+lemma lift_by_succ {a} (t : preterm σ a) {m i} : t ↑ (m+1) ＠ i  = (t ↑ 1 ＠ i) ↑ m ＠ i
   := begin rw[lift_lift_merge, one_add], apply le_refl, apply le_succ, end
 
-/-
-  Another common operation on the environment comes in the form of substitution.
-  For example, this is the case whenever we write "Let xₖ = s" in a proof.
-  Substituting `s` for `xₖ` in a term `t`, naively, should replace each
-  variable at `k` by `s`.
-  One obvious problem is that `s` could still be referencing `xₖ`.
-  We can avoid this by informally removing `xₖ` from the environment,
-  i.e. by decreasing each `k+1`-free variable during substitution by 1.
-  Another thing to consider is that the variables bound by `xₖ` 
-  are by definition `k`-free,  while this is not necessarily true for the term `s`. 
 
-  If we imagine our environment as a timeline objects we have defined or constructed,
-  then each `xₖ` should only depend on the objects `...,xₖ₊₂,xₖ₊₁` that came before.
-  Naive substitution however breaks the chronology of this timeline.
-
-  Thus, to ensure we replace a `k`-free term by another `k`-free term (and keep chronology), 
-  we define a form of capture-free substitution as below.
--/
 
 /-- 
   `subst t s k` substitutes `s ↑ k ＠ 0` for each variable at `k` in `t` and 
   reduces the index of all `k+1`-free variables by `1`.
 -/
-def subst: ∀{a}, preterm 𝒮 a → term 𝒮 → ℕ → preterm 𝒮 a
+def subst: ∀{a}, preterm σ a → term σ → ℕ → preterm σ a
 | _ #x           s k := if x < k then #x else if k < x then #(x-1) else (s ↑ k ＠ 0)
 | _ (func f)     s k := func f
 | _ (fapp t₁ t₂) s k := fapp (subst t₁ s k) (subst t₂ s k)
@@ -248,37 +177,35 @@ def subst: ∀{a}, preterm 𝒮 a → term 𝒮 → ℕ → preterm 𝒮 a
 end term
 
 -- we use ⁄ (U+2044) instead of the usual slash / (U+002F) to avoid conflict with the division operator
--- recommended to make a custom shortcut as the default \textfractionsolidus is quite unhandy
 notation t `[`:max s ` ⁄ `:95 n `]`:0 := term.subst t s n 
--- #reduce #5[#2 ⁄ 1]
 
 namespace term
 
 -- lemmas for the simplifier
-@[simp, tls] lemma subst_fapp {a} (t₁ : preterm 𝒮 (a+1)) (t₂ s : preterm 𝒮 0) (k : ℕ ) : 
+@[simp, tls] lemma subst_fapp {a} (t₁ : preterm σ (a+1)) (t₂ s : preterm σ 0) (k : ℕ) : 
   (fapp t₁ t₂) [s ⁄ k] = fapp (t₁ [s ⁄ k]) (t₂ [s ⁄ k]) := by refl
-@[simp, tls] lemma subst_func {a} (f : 𝒮.func_symb a) (s k) : 
+@[simp, tls] lemma subst_func {a} (f : σ.func_symb a) (s k) : 
   (func f) [s ⁄ k] = func f := by refl
 
-@[simp] lemma subst_var_lt (s : term 𝒮) {x k : ℕ} (H : x < k) : #x[s ⁄ k] = #x := 
+@[simp] lemma subst_var_lt (s : term σ) {x k : ℕ} (H : x < k) : #x[s ⁄ k] = #x := 
     begin rw subst, rw if_pos H, end
-@[simp, tls] lemma subst_var_eq (s : term 𝒮) {k : ℕ}  : #k[s ⁄ k] =  s ↑ k ＠ 0 := 
+@[simp, tls] lemma subst_var_eq (s : term σ) {k : ℕ}  : #k[s ⁄ k] =  s ↑ k ＠ 0 := 
     begin rw subst, repeat{ rw if_neg (lt_irrefl k) }, end
-@[simp] lemma subst_var_gt (s : term 𝒮) {x k  : ℕ} (H : k < x) : #x[s ⁄ k] = #(x-1) := 
+@[simp] lemma subst_var_gt (s : term σ) {x k  : ℕ} (H : k < x) : #x[s ⁄ k] = #(x-1) := 
     begin rw subst, rw if_neg (lt_asymm H), rw if_pos H, end
-@[simp] lemma subst_var_nle (s : term 𝒮) {x k : ℕ} (H : ¬ (x ≤ k)) : #x[s ⁄ k] = #(x-1) := 
+@[simp] lemma subst_var_nle (s : term σ) {x k : ℕ} (H : ¬ (x ≤ k)) : #x[s ⁄ k] = #(x-1) := 
   subst_var_gt s (not_le.mp H)
 
-@[simp, tls] lemma subst_var0 (s : term 𝒮): #0[ s ⁄ 0 ] = s := 
+@[simp, tls] lemma subst_var0 (s : term σ): #0[ s ⁄ 0 ] = s := 
     begin rw subst_var_eq, exact lift_by_0 s, end
 
 
--- substitution lemmas
-lemma lift_subst : ∀ {a}  (t : preterm 𝒮 a) (s: term 𝒮) (m) {i} (k) ( H: i ≤ k ),
-    t [ s ⁄ k ] ↑ m ＠ i = (t ↑ m ＠ i )[ s ⁄ k+m ] 
+/- Various substitution lemmas -/
+
+lemma lift_subst : ∀ {a}  (t : preterm σ a) (s: term σ) (m) {i} (k) (H: i ≤ k),
+    t [ s ⁄ k ] ↑ m ＠ i = (t ↑ m ＠ i)[ s ⁄ k+m ] 
 | _ #x s m i k H := 
   begin 
-    --unfold subst lift,
     apply decidable.lt_by_cases x k; intro h₁,
     { -- x < k
       have h₂ : x < k + m, from nat.lt_add_right x k m h₁, by_cases i≤x;
@@ -288,16 +215,15 @@ lemma lift_subst : ∀ {a}  (t : preterm 𝒮 a) (s: term 𝒮) (m) {i} (k) ( H:
       simp[*, lift_lift_merge] , } ,
     { -- x > k
       have h₂ : i < x, by linarith,
-      have : i ≤ x-1, from nat.le_sub_right_of_add_le (succ_le_of_lt h₂ ),
+      have : i ≤ x-1, from nat.le_sub_right_of_add_le (succ_le_of_lt h₂),
       have : i ≤ x, by linarith,
       have : 1 ≤ x, by linarith,
-      simp[*, nat.sub_add_comm],
-    },
+      simp[*, nat.sub_add_comm] },
   end
 | _ (func f)   _ _ _ _ _ := by refl
 | _ (fapp f t) _ _ _ _ _ := by simp* 
 
-lemma subst_lift: ∀  {a}  (t : preterm 𝒮 a) (s: term 𝒮) {m i k : ℕ} (H: i ≤ k) (H' : k ≤ i + m),
+lemma subst_lift: ∀  {a}  (t : preterm σ a) (s: term σ) {m i k : ℕ} (H: i ≤ k) (H' : k ≤ i + m),
     (t ↑ (m+1) ＠ i) [s ⁄ k] = t ↑ m ＠ i 
 | _ #x s m i k H H' := 
   begin by_cases h: i ≤ x,
@@ -307,7 +233,7 @@ lemma subst_lift: ∀  {a}  (t : preterm 𝒮 a) (s: term 𝒮) {m i k : ℕ} (H
 | _ (func f)   _ _ _ _ _ _ := by refl
 | _ (fapp f t) _ _ _ _ _ _ := by simp* 
 
-lemma subst_subst: ∀ {a} (t : preterm 𝒮 a) (s₁) {k₁}  (s₂) {k₂} (H : k₁ ≤ k₂), 
+lemma subst_subst: ∀ {a} (t : preterm σ a) (s₁) {k₁}  (s₂) {k₂} (H : k₁ ≤ k₂), 
     t[s₁ ⁄ k₁][s₂ ⁄ k₂] = t[s₂ ⁄ k₂ + 1][(s₁ [s₂ ⁄ k₂ - k₁]) ⁄ k₁] 
 | _ #x s₁ k₁ s₂ k₂ H := 
   begin apply decidable.lt_by_cases x k₁; intro h₁,
@@ -318,12 +244,11 @@ lemma subst_subst: ∀ {a} (t : preterm 𝒮 a) (s₁) {k₁}  (s₂) {k₂} (H 
       have h₂ : x < k₂ + 1, from lt_succ_iff.mpr H,
       simp[*, lift_subst, nat.sub_add_cancel] , },
     { apply decidable.lt_by_cases (x-1) k₂; intro h₂,
-      { have : x < k₂ + 1, from nat.lt_add_of_sub_lt_right h₂, simp[*] , },
+      { have : x < k₂ + 1, from nat.lt_add_of_sub_lt_right h₂, simp*, },
       { have h₃: 1 ≤  x , from by linarith,
         have h₄: x  = k₂ + 1, from (nat.sub_eq_iff_eq_add h₃).mp h₂,
         subst h₄, clear h₃,
-        simp[*, subst_lift, lt_irrefl] , 
-      },
+        simp[*, subst_lift, lt_irrefl] },
       { have: k₂+1 < x,   from nat.add_lt_of_lt_sub_right h₂, 
         have: k₁ < x - 1, from gt_of_gt_of_ge h₂ H,
         simp[*], }, }, 
@@ -331,8 +256,8 @@ lemma subst_subst: ∀ {a} (t : preterm 𝒮 a) (s₁) {k₁}  (s₂) {k₂} (H 
 | _ (func f) _ _ _ _ _ := by refl
 | _ (fapp t s) _ _ _ _ _ := by simp*
 
-lemma subst_lift_by_lift : ∀{a} (t : preterm 𝒮 a) (s : term 𝒮) (m i k : ℕ),
-    (t ↑ m ＠ ( i + k + 1 ) ) [ (s ↑ m ＠ i) ⁄ k] = (t [ s ⁄ k ]) ↑ m ＠ (i+k)
+lemma subst_lift_by_lift : ∀{a} (t : preterm σ a) (s : term σ) (m i k : ℕ),
+    (t ↑ m ＠ (i + k + 1)) [ (s ↑ m ＠ i) ⁄ k] = (t [ s ⁄ k ]) ↑ m ＠ (i+k)
 | _ #x s m i k :=
   begin by_cases h₁ : i + k + 1 ≤ x,
     { -- i + k + 1 ≤ x
@@ -360,7 +285,7 @@ lemma subst_lift_by_lift : ∀{a} (t : preterm 𝒮 a) (s : term 𝒮) (m i k : 
 | _ (func f)     _ _ _ _ := by refl
 | _ (fapp t₁ t₂) _ _ _ _ := by simp* 
 
-lemma subst_var0_lift : ∀{a} (t : preterm 𝒮 a) (m i : ℕ), (t ↑ (m+1) ＠  (i+1) )[ #0 ⁄ i] = t ↑ m ＠ (i+1)
+lemma subst_var0_lift : ∀{a} (t : preterm σ a) (m i : ℕ), (t ↑ (m+1) ＠ (i+1))[ #0 ⁄ i] = t ↑ m ＠ (i+1)
 | _ #x m i := begin apply decidable.lt_by_cases i x; intro h₀,
                 { have: i+1 ≤ x, by linarith,
                   have: ¬ (x + (m + 1) < i), by linarith, 
@@ -372,18 +297,17 @@ lemma subst_var0_lift : ∀{a} (t : preterm 𝒮 a) (m i : ℕ), (t ↑ (m+1) �
 | _ (func f) _ _ := by refl
 | _ (fapp t s) _ _ := by simp* 
 
-@[simp, tls] lemma subst_var0_lift_by_1 {a} (t : preterm 𝒮 a) (i : ℕ) : (t ↑ (1) ＠  (i+1) )[#0 ⁄ i] = t := 
+@[simp, tls] lemma subst_var0_lift_by_1 {a} (t : preterm σ a) (i : ℕ) : (t ↑ (1) ＠ (i+1))[#0 ⁄ i] = t := 
 begin
     have h:= subst_var0_lift t 0 i,
     rw lift_by_0 at h,
     exact h,
 end
 
-@[simp, tls] lemma subst_for_0_lift_by_1: ∀ {a} (t : preterm 𝒮 a) (s : term 𝒮) , (t ↑ 1 ＠ 0 )[s ⁄ 0] = t 
+@[simp, tls] lemma subst_for_0_lift_by_1: ∀ {a} (t : preterm σ a) (s : term σ) , (t ↑ 1 ＠ 0)[s ⁄ 0] = t 
 | _ #x _         := by refl
 | _ (func f) _   := by refl
 | _ (fapp t s) _ := by simp* 
-
 
 /--
   Biggest (deepest) reference depth of variables occurring in a term (plus one).
@@ -392,13 +316,13 @@ end
   * `max_free_var #k = k+1` by definition.
   * `max_free_var t = 0` means no variables occur in `t`.
 -/
-def max_free_var: ∀ {a} (t : preterm 𝒮 a), ℕ 
+def max_free_var: ∀ {a} (t : preterm σ a), ℕ 
 | _ #x := x+1
 | _ (func f)  := 0
 | _ (fapp t s) := max (max_free_var t) (max_free_var s)
 
-/- If `t` is a fixpoint for lifting at `i`, then its a fixpoint for lifting at `j` for all `i≤j`  -/
-lemma trivial_lift_monotone {a} {t:preterm 𝒮 a} {i j: ℕ} (h: i ≤ j) (H: t ↑ 1 ＠ i = t) : t ↑ 1 ＠ j = t :=
+/- If `t` is a fixed point for lifting at `i`, then its a fixed point for lifting at `j` for all `i≤j`  -/
+lemma lift_fixed_points_monotone {a} {t:preterm σ a} {i j: ℕ} (h: i ≤ j) (H: t ↑ 1 ＠ i = t) : t ↑ 1 ＠ j = t :=
 begin
   induction j with j,
   { rwa[le_zero_iff.mp h] at H,},
@@ -410,7 +334,7 @@ begin
   },
 end
 
-@[simp, tls] lemma lift_at_max_free_var {a} (t : preterm 𝒮 a) : t ↑ 1 ＠ (max_free_var t) = t :=
+@[simp, tls] lemma lift_at_max_free_var {a} (t : preterm σ a) : t ↑ 1 ＠ (max_free_var t) = t :=
 begin
   induction t with T,
   { simp[max_free_var], },
@@ -418,36 +342,35 @@ begin
   { unfold lift max_free_var,
     congr,
     { have t_h := le_max_left (max_free_var t_t) (max_free_var t_s),
-      exact trivial_lift_monotone t_h t_ih_t, },
+      exact lift_fixed_points_monotone t_h t_ih_t, },
     { have s_h := le_max_right (max_free_var t_t) (max_free_var t_s),
-      exact trivial_lift_monotone s_h t_ih_s, } }
+      exact lift_fixed_points_monotone s_h t_ih_s, } }
 end 
 
 end term
 
-
 /-! ### formulas -/
 section formulas
 
-variable (𝒮)
+variable (σ)
 /--
-  `preformula 𝒮 a` is a partially applied formula of first-order logic over the signature `𝒮`. 
+  `preformula σ a` is a partially applied formula of first-order logic over the signature `σ`. 
   If applied to `a` terms it becomes a well-formed formula.
 -/
 inductive preformula : ℕ → Type u
 | bot                           : preformula 0
-| eq   ( t s : term 𝒮 )         : preformula 0
-| imp  ( φ ψ : preformula 0 )   : preformula 0
-| and  ( φ ψ : preformula 0 )   : preformula 0
-| or   ( φ ψ : preformula 0 )   : preformula 0
-| all  ( φ : preformula 0 )     : preformula 0
-| ex   ( φ : preformula 0 )     : preformula 0 
-| pred { arity : ℕ } ( P : 𝒮.pred_symb arity )                  : preformula arity 
-| papp { arity : ℕ } ( φ : preformula (arity+1) ) ( t : term 𝒮 ) : preformula arity
+| eq   (t s : term σ)         : preformula 0
+| imp  (φ ψ : preformula 0)   : preformula 0
+| and  (φ ψ : preformula 0)   : preformula 0
+| or   (φ ψ : preformula 0)   : preformula 0
+| all  (φ : preformula 0)     : preformula 0
+| ex   (φ : preformula 0)     : preformula 0 
+| pred {arity : ℕ} (P : σ.pred_symb arity)                  : preformula arity 
+| papp {arity : ℕ} (φ : preformula (arity+1)) (t : term σ) : preformula arity
 
-@[reducible] def formula := preformula 𝒮 0
+@[reducible] def formula := preformula σ 0
 
-variable {𝒮}
+variable {σ}
 
 notation `⊥'`     := preformula.bot 
 infix ` =' `:100  := preformula.eq  
@@ -459,75 +382,46 @@ infixr ` ∧' `:90  := preformula.and
 prefix `∀'`:110   := preformula.all
 prefix `∃'`:110   := preformula.ex 
 
-@[simp] def preformula.iff (φ ψ : formula 𝒮) : formula 𝒮 := (φ →' ψ) ∧' (ψ  →' φ)
+@[simp] def preformula.iff (φ ψ : formula σ) : formula σ := (φ →' ψ) ∧' (ψ  →' φ)
 infix ` ↔' `:70 := preformula.iff -- input \<=>
 
-@[simp] def preformula.not (φ : formula 𝒮) : formula 𝒮 := (φ →' ⊥') 
+@[simp] def preformula.not (φ : formula σ) : formula σ := (φ →' ⊥') 
 prefix `¬'`:115 := preformula.not
 
-def preformula.top : formula 𝒮  := ¬' ⊥'
+def preformula.top : formula σ  := ¬' ⊥'
 notation `⊤'` := preformula.top
 
 export preformula
-
-/- 
-  ## Definition
-  The variables of a formula `φ` are by structural induction in the obvious way.
-
-  The variables at reference depth `k` or simply at `k` are defined 
-  by structural induction as follows:
-  - `⊥` and `pred P` have no variables at `k`
-  the variables at `k` of 
-  - `t=s`      are the variables at `k` of `t` and of `s`
-  - `φ □ ψ`    are the variables at `k` of `φ` and of `ψ` for `□ ∈ { → , ∧ , ∨ }`
-  - `papp φ t` are the variables at `k` of `φ` and of `t`
-  And most importantly 
-  - `□ φ`      are the variables at `k+1` of `φ` for `□ ∈ { ∀, ∃ }`
-
-  A variable of `φ` is called `k`-free if it is at a reference depth `≥k`.
-  
-  ## Remark
-  It follows that quantifiers act as another form of variable binders,
-  this time not just imagined. 
-  To define lifting (resp. substitution) of formulas we therefore need 
-  to increase the reference depth at which we lift (resp. substitute)
-  at whenever we cross a quantifier.
-
-  With this we can directly translate the lifting and substitution
-  lemmas of terms to formulas and their proofs will generally reduce to
-  the respective lemmas for terms (and some light arithmetic for crossing quantifiers).
--/
 
 section lifts_and_substitutions
 
 namespace formula
 
 /-- `lift φ m i` increases the index of `i`-free variables in `φ` by `m`. -/
-@[simp, reducible] def lift : ∀{a} , preformula 𝒮 a → ℕ → ℕ → preformula 𝒮 a 
+@[simp, reducible] def lift : ∀{a} , preformula σ a → ℕ → ℕ → preformula σ a 
 | _ ⊥'  _ _         := ⊥'  
 | _ (t =' s) m i    := (term.lift t m i) =' (term.lift s m i)
-| _ ( φ →' ψ ) m i  := (lift φ m i) →' (lift ψ  m i)
-| _ ( φ ∧' ψ ) m i  := (lift φ m i) ∧' (lift ψ  m i)
-| _ ( φ ∨' ψ ) m i  := (lift φ m i) ∨' (lift ψ  m i)
-| _ ( ∀' φ ) m i    := ∀' (lift φ m (i+1))
-| _ ( ∃' φ ) m i    := ∃' (lift φ m (i+1))
+| _ (φ →' ψ) m i  := (lift φ m i) →' (lift ψ  m i)
+| _ (φ ∧' ψ) m i  := (lift φ m i) ∧' (lift ψ  m i)
+| _ (φ ∨' ψ) m i  := (lift φ m i) ∨' (lift ψ  m i)
+| _ (∀' φ) m i    := ∀' (lift φ m (i+1))
+| _ (∃' φ) m i    := ∃' (lift φ m (i+1))
 | _ (pred P) _ _    := pred P
 | _ (papp φ t) m i  := papp (lift φ m i) (term.lift t m i)
 
 /-- `subst t s k` substitutes `s ↑ k ＠ 0` for each variable at `k` in `t` -/
-@[simp, tls] def subst :  ∀{a} , preformula 𝒮 a → term 𝒮 → ℕ → preformula 𝒮 a
+@[simp, tls] def subst :  ∀{a} , preformula σ a → term σ → ℕ → preformula σ a
 | _ ⊥'  _ _         := ⊥'  
-| _ ( t₁ =' t₂) s k := (term.subst t₁ s k) =' (term.subst t₂ s k)
-| _ ( φ →' ψ ) s k  := (subst φ s k) →' (subst ψ  s k)
-| _ ( φ ∧' ψ ) s k  := (subst φ s k) ∧' (subst ψ  s k)
-| _ ( φ ∨' ψ ) s k  := (subst φ s k) ∨' (subst ψ  s k)
-| _ ( ∀' φ ) s k    := ∀' (subst φ  s (k+1))
-| _ ( ∃' φ ) s k    := ∃' (subst φ  s (k+1))
+| _ (t₁ =' t₂) s k := (term.subst t₁ s k) =' (term.subst t₂ s k)
+| _ (φ →' ψ) s k  := (subst φ s k) →' (subst ψ  s k)
+| _ (φ ∧' ψ) s k  := (subst φ s k) ∧' (subst ψ  s k)
+| _ (φ ∨' ψ) s k  := (subst φ s k) ∨' (subst ψ  s k)
+| _ (∀' φ) s k    := ∀' (subst φ  s (k+1))
+| _ (∃' φ) s k    := ∃' (subst φ  s (k+1))
 | _ (pred P) _ _    := pred P
 | _ (papp φ t) s k  := papp (subst φ s k) (term.subst t s k)
 
 end formula
-
 
 notation f ` ↑ `:90 m ` ＠ `:90 i :90 := formula.lift f m i
 notation φ `[`:max t ` ⁄ `:95 n `]`:0 := formula.subst φ t n
@@ -541,147 +435,152 @@ namespace formula
 open preformula
 
 -- lift and substitution lemmas for formulas
-@[simp, tls] lemma lift_by_0: ∀ {a} ( φ : preformula 𝒮 a) {i}, φ ↑ 0 ＠ i = φ
-| _ ⊥' _            := by refl
-| _ (t =' s) _      := by simp
-| _ ( φ →' ψ ) _    := begin rw lift, congr; exact lift_by_0 _, end
-| _ ( φ ∧' ψ ) _    := begin rw lift, congr; exact lift_by_0 _, end
-| _ ( φ ∨' ψ ) _    := begin rw lift, congr; exact lift_by_0 _, end
-| _ ( ∀' φ ) _      := begin rw lift, congr, exact lift_by_0 φ, end
-| _ ( ∃' φ ) _      := begin rw lift, congr, exact lift_by_0 φ, end
-| _ ( pred P ) _    := by refl
-| _ ( papp φ t ) _  := begin rw lift, congr, exact lift_by_0 φ, exact term.lift_by_0 t, end
+@[simp, tls] lemma lift_by_0: ∀ {a} (φ : preformula σ a) {i}, φ ↑ 0 ＠ i = φ
+| _ ⊥' _          := by refl
+| _ (t =' s) _    := by simp
+| _ (φ →' ψ) _    := begin rw lift, congr; exact lift_by_0 _, end
+| _ (φ ∧' ψ) _    := begin rw lift, congr; exact lift_by_0 _, end
+| _ (φ ∨' ψ) _    := begin rw lift, congr; exact lift_by_0 _, end
+| _ (∀' φ) _      := begin rw lift, congr, exact lift_by_0 φ, end
+| _ (∃' φ) _      := begin rw lift, congr, exact lift_by_0 φ, end
+| _ (pred P) _    := by refl
+| _ (papp φ t) _  := begin rw lift, congr, exact lift_by_0 φ, exact term.lift_by_0 t, end
 
-lemma lift_lift: ∀{a} ( φ : preformula 𝒮 a) (m) {i} (n) {j} ( H : j ≤ i ),
+lemma lift_lift: ∀{a} (φ : preformula σ a) (m) {i} (n) {j} (H : j ≤ i),
     (φ ↑ m ＠ i) ↑ n ＠ j = (φ ↑ n ＠ j) ↑ m ＠ (i+n)   
-| _ ⊥' _ _ _ _ _             := by refl
-| _ ( t =' s ) _ _ _ _ _     := by simp[*, term.lift_lift]
-| _ ( φ →' ψ ) _ _ _ _ _     := by simp[*]
-| _ ( φ ∧' ψ ) _ _ _ _ _     := by simp[*]
-| _ ( φ ∨' ψ ) _ _ _ _ _     := by simp[*]
-| _ ( ∀' φ ) _ _ _ _ _       := by simp[*, add_right_comm]
-| _ ( ∃' φ ) _ _ _ _ _       := by simp[*, add_right_comm]
-| _ ( pred P ) _ _ _ _ _     := by refl
-| _ ( papp φ t ) _ _ _ _ _   := by simp[*, term.lift_lift]
+| _ ⊥' _ _ _ _ _           := by refl
+| _ (t =' s) _ _ _ _ _     := by simp[*, term.lift_lift]
+| _ (φ →' ψ) _ _ _ _ _     := by simp[*]
+| _ (φ ∧' ψ) _ _ _ _ _     := by simp[*]
+| _ (φ ∨' ψ) _ _ _ _ _     := by simp[*]
+| _ (∀' φ) _ _ _ _ _       := by simp[*, add_right_comm]
+| _ (∃' φ) _ _ _ _ _       := by simp[*, add_right_comm]
+| _ (pred P) _ _ _ _ _     := by refl
+| _ (papp φ t) _ _ _ _ _   := by simp[*, term.lift_lift]
 
-lemma lift_lift_reverse {a} ( φ : preformula 𝒮 a) {m i} (n) {j} (H : i + m ≤ j) :
-    (φ ↑ m ＠ i) ↑ n ＠ j = (φ  ↑ n ＠  (j-m)) ↑ m ＠ i := 
+lemma lift_lift_reverse {a} (φ : preformula σ a) {m i} (n) {j} (H : i + m ≤ j) :
+    (φ ↑ m ＠ i) ↑ n ＠ j = (φ ↑ n ＠ (j-m)) ↑ m ＠ i := 
 begin
     have h : i ≤ (j-m), from nat.le_sub_right_of_add_le H,
     have h': m ≤ j, from (le_trans (m.le_add_left i) H),
     rw [lift_lift φ n m h, nat.sub_add_cancel h'],
 end
 
-lemma lift_lift_merge: ∀ {a} ( φ : preformula 𝒮 a ) {m i} (n) {j} (H : i ≤ j) (H' : j ≤ i + m),
+lemma lift_lift_merge: ∀ {a} (φ : preformula σ a) {m i} (n) {j} (H : i ≤ j) (H' : j ≤ i + m),
     (φ ↑ m ＠ i) ↑ n ＠ j = φ ↑ (m+n) ＠ i
-| _ ⊥' _ _ _ _ _ _           := by refl 
-| _ ( t =' s) _ _ _ _ _ _    := by simp[*, term.lift_lift_merge]
-| _ ( φ →' ψ ) _ _ _ _ _ _   := by simp[*]
-| _ ( φ ∧' ψ ) _ _ _ _ _ _   := by simp[*]
-| _ ( φ ∨' ψ ) _ _ _ _ _ _   := by simp[*]
-| _ ( ∀' φ ) _ _ _ _ _ _     := by simp[*, add_right_comm]
-| _ ( ∃' φ ) _ _ _ _ _ _     := by simp[*, add_right_comm]
-| _ ( pred P ) _ _ _ _ _ _   := by refl
-| _ ( papp φ t ) _ _ _ _ _ _ := by simp[*, term.lift_lift_merge]
+| _ ⊥' _ _ _ _ _ _         := by refl 
+| _ (t =' s) _ _ _ _ _ _   := by simp[*, term.lift_lift_merge]
+| _ (φ →' ψ) _ _ _ _ _ _   := by simp[*]
+| _ (φ ∧' ψ) _ _ _ _ _ _   := by simp[*]
+| _ (φ ∨' ψ) _ _ _ _ _ _   := by simp[*]
+| _ (∀' φ) _ _ _ _ _ _     := by simp[*, add_right_comm]
+| _ (∃' φ) _ _ _ _ _ _     := by simp[*, add_right_comm]
+| _ (pred P) _ _ _ _ _ _   := by refl
+| _ (papp φ t) _ _ _ _ _ _ := by simp[*, term.lift_lift_merge]
 
-@[simp, tls] lemma lift_at_lift_merge {a} ( φ : preformula 𝒮 a ) (m i n):
-    ( φ ↑ m ＠ i ) ↑ n ＠ i = φ ↑ (m+n) ＠ i := lift_lift_merge φ n (le_rfl) (i.le_add_right m)
+@[simp, tls] lemma lift_at_lift_merge {a} (φ : preformula σ a) (m i n):
+    (φ ↑ m ＠ i) ↑ n ＠ i = φ ↑ (m+n) ＠ i := lift_lift_merge φ n (le_rfl) (i.le_add_right m)
 
 lemma lambda_lift_lift {a} (m) {i} (n) {j} (H : j≤i) : 
-    (λ ( φ :preformula 𝒮 a),  ( φ ↑ m ＠ i ) ↑ n ＠ j ) = (λ φ, ( φ ↑ n ＠ j) ↑ m ＠ (i+n)) :=
+    (λ (φ :preformula σ a),  (φ ↑ m ＠ i) ↑ n ＠ j) = (λ φ, (φ ↑ n ＠ j) ↑ m ＠ (i+n)) :=
 begin funext, apply lift_lift, exact H, end
 
-lemma lift_subst: ∀ {a}  (φ : preformula 𝒮 a) (s: term 𝒮) ( m i k : ℕ ) (h': i ≤ k),
-     φ[s ⁄ k] ↑ m ＠ i = (φ ↑ m ＠  i)[s ⁄ (k+m)]  
-| _ ⊥' _ _ _ _ _            := by refl
-| _ (t₁ =' t₂) _ _ _ _ _    := by simp[*, term.lift_subst]
-| _ ( φ →' ψ ) _ _ _ _ _    := by simp[*]
-| _ ( φ ∧' ψ ) _ _ _ _ _    := by simp[*]
-| _ ( φ ∨' ψ ) _ _ _ _ _    := by simp[*]
-| _ ( ∀' φ ) _ _ _ _ _      := by simp[*, add_right_comm]
-| _ ( ∃' φ ) _ _ _ _ _      := by simp[*, add_right_comm]
-| _ ( pred P ) _ _ _ _ _    := by refl
-| _ ( papp φ t ) _ _ _ _ _  := by simp[*, term.lift_subst]
+lemma lift_subst: ∀ {a}  (φ : preformula σ a) (s: term σ) (m i k : ℕ) (h': i ≤ k),
+     φ[s ⁄ k] ↑ m ＠ i = (φ ↑ m ＠ i)[s ⁄ (k+m)]  
+| _ ⊥' _ _ _ _ _          := by refl
+| _ (t₁ =' t₂) _ _ _ _ _  := by simp[*, term.lift_subst]
+| _ (φ →' ψ) _ _ _ _ _    := by simp[*]
+| _ (φ ∧' ψ) _ _ _ _ _    := by simp[*]
+| _ (φ ∨' ψ) _ _ _ _ _    := by simp[*]
+| _ (∀' φ) _ _ _ _ _      := by simp[*, add_right_comm]
+| _ (∃' φ) _ _ _ _ _      := by simp[*, add_right_comm]
+| _ (pred P) _ _ _ _ _    := by refl
+| _ (papp φ t) _ _ _ _ _  := by simp[*, term.lift_subst]
 
-lemma subst_lift : ∀ {a}  ( φ : preformula 𝒮 a) (s: term 𝒮) {m i k : ℕ } (H: i ≤ k) (H' : k ≤ i + m),
+lemma lambda_lift_subst_formula {a} {s: term σ} { m i k : ℕ } (h': i ≤ k) :
+  (λ (ϕ: preformula σ a), lift (subst ϕ s k) m i) = (λ ϕ, subst (lift ϕ m i) s (k+m)) :=
+begin funext, apply lift_subst, assumption, end
+
+lemma subst_lift : ∀ {a}  (φ : preformula σ a) (s: term σ) {m i k : ℕ } (H: i ≤ k) (H' : k ≤ i + m),
     (φ ↑ (m+1) ＠ i)[s ⁄ k] = φ ↑ m ＠ i 
 | _ ⊥' _ _ _ _ _ _          := by refl
 | _ (t₁ =' t₂) _ _ _ _ _ _  := by simp[*, term.subst_lift]
-| _ ( φ →' ψ ) _ _ _ _ _ _  := by simp[*]
-| _ ( φ ∧' ψ ) _ _ _ _ _ _  := by simp[*]
-| _ ( φ ∨' ψ ) _ _ _ _ _ _  := by simp[*]
-| _ ( ∀' φ ) _ _ _ _ _ _    := by simp[*, add_right_comm]
-| _ ( ∃' φ ) _ _ _ _ _ _    := by simp[*, add_right_comm]
+| _ (φ →' ψ) _ _ _ _ _ _  := by simp[*]
+| _ (φ ∧' ψ) _ _ _ _ _ _  := by simp[*]
+| _ (φ ∨' ψ) _ _ _ _ _ _  := by simp[*]
+| _ (∀' φ) _ _ _ _ _ _    := by simp[*, add_right_comm]
+| _ (∃' φ) _ _ _ _ _ _    := by simp[*, add_right_comm]
 | _ (pred P) _ _ _ _ _ _    := by refl
-| _ ( papp φ t) _ _ _ _ _ _ := by simp[*, term.subst_lift]
+| _ (papp φ t) _ _ _ _ _ _ := by simp[*, term.subst_lift]
 
-lemma subst_subst : ∀ {a} ( φ : preformula 𝒮 a) (s₁) {k₁} (s₂) {k₂} ( H : k₁ ≤ k₂ ), 
-    φ [ s₁ ⁄ k₁] [ s₂ ⁄ k₂] = φ [ s₂ ⁄ k₂ + 1] [ (s₁ [s₂ ⁄ k₂ - k₁] ) ⁄ k₁ ] 
-| _ ⊥' _ _ _ _ _            := by refl
-| _ (t₁ =' t₂) _ _ _ _ _    := by simp[*, term.subst_subst]
-| _ ( φ →' ψ ) _ _ _ _ _    := by simp[*]
-| _ ( φ ∧' ψ ) _ _ _ _ _    := by simp[*]
-| _ ( φ ∨' ψ ) _ _ _ _ _    := by simp[*]
-| _ ( ∀' φ ) _ _ _ _ _      := by simp[*, add_right_comm]
-| _ ( ∃' φ ) _ _ _ _ _      := by simp[*, add_right_comm]
-| _ (pred P) _ _ _ _ _      := by refl
-| _ (papp φ t) _ _ _ _ _    := by simp[*, term.subst_subst]
-
-lemma subst_lift_in_lift : ∀{a} ( φ : preformula 𝒮 a) (s : term 𝒮) (m i k),
+lemma subst_lift_in_lift : ∀{a} (φ : preformula σ a) (s : term σ) (m i k),
     (φ ↑ m ＠ (i + k + 1)) [ (s ↑ m ＠ i) ⁄ k] = φ[s ⁄ k] ↑ m ＠ (i+k) 
-| _ ⊥' _ _ _ _          := by refl
-| _ (t₁ =' t₂) _ _ _ _  := by simp[*, term.subst_lift_by_lift]
-| _ ( φ →' ψ ) _ _ _ _  := by simp[*]
-| _ ( φ ∧' ψ ) _ _ _ _  := by simp[*]
-| _ ( φ ∨' ψ ) _ _ _ _  := by simp[*]
-| _ (∀' φ ) s m i k     := begin have := subst_lift_in_lift φ s m i (k+1), rw[add_succ i k] at this, simp[*, add_right_comm], end
-| _ (∃' φ ) s m i k     := begin have := subst_lift_in_lift φ s m i (k+1), rw[add_succ i k] at this, simp[*, add_right_comm], end
-| _ (pred P) _ _ _ _    := by refl
-| _ (papp φ t) _ _ _ _  := by simp[*, term.subst_lift_by_lift]
+| _ ⊥' _ _ _ _         := by refl
+| _ (t₁ =' t₂) _ _ _ _ := by simp[*, term.subst_lift_by_lift]
+| _ (φ →' ψ) _ _ _ _   := by simp[*]
+| _ (φ ∧' ψ) _ _ _ _   := by simp[*]
+| _ (φ ∨' ψ) _ _ _ _   := by simp[*]
+| _ (∀' φ) s m i k     := begin have := subst_lift_in_lift φ s m i (k+1), rw[add_succ i k] at this, simp[*, add_right_comm], end
+| _ (∃' φ) s m i k     := begin have := subst_lift_in_lift φ s m i (k+1), rw[add_succ i k] at this, simp[*, add_right_comm], end
+| _ (pred P) _ _ _ _   := by refl
+| _ (papp φ t) _ _ _ _ := by simp[*, term.subst_lift_by_lift]
 
 
-@[tls] lemma subst0_lift_by_lift {a}  (φ : preformula 𝒮 a) {s : term 𝒮} {m i:ℕ } :
-    (φ ↑ m ＠ (i + 1)) [(s ↑ m ＠ i) ⁄ 0] = φ[s ⁄ 0] ↑ m ＠ i := subst_lift_in_lift φ s m i 0
+@[tls] lemma subst0_lift_by_lift {a}  (φ : preformula σ a) {s : term σ} {m i:ℕ } :
+  (φ ↑ m ＠ (i + 1)) [(s ↑ m ＠ i) ⁄ 0] = φ[s ⁄ 0] ↑ m ＠ i := subst_lift_in_lift φ s m i 0
 
-@[tls] lemma subst_at_lift {a} (φ : preformula 𝒮 a) (m) (s : term 𝒮) (k) : 
+@[tls] lemma subst_at_lift {a} (φ : preformula σ a) (m) (s : term σ) (k) : 
   (φ ↑ (m+1) ＠ k)[s ⁄ k] =  φ ↑ m ＠ k := subst_lift φ s (le_refl k) (le.intro rfl)
 
-@[tls] lemma subst_var0_lift : ∀{a} (φ : preformula 𝒮 a) (m i : ℕ), 
+@[tls] lemma subst_var0_lift : ∀{a} (φ : preformula σ a) (m i : ℕ), 
   (φ ↑ (m+1) ＠ (i+1))[#0 ⁄ i] = φ ↑ m ＠ (i+1)
-| _ ⊥'  _ _         := by refl 
-| _ ( t₁ =' t₂) m i := by simp[term.subst_var0_lift]
-| _ ( φ →' ψ ) m i  := by simp*
-| _ ( φ ∧' ψ ) m i  := by simp*
-| _ ( φ ∨' ψ ) m i  := by simp*
-| _ ( ∀' φ ) m i    := by simp*
-| _ ( ∃' φ ) m i    := by simp*
-| _ (pred P) _ _    := by refl
-| _ (papp φ t) m i  := by simp[*, term.subst_var0_lift]
+| _ ⊥'  _ _        := by refl 
+| _ (t₁ =' t₂) m i := by simp[term.subst_var0_lift]
+| _ (φ →' ψ) m i   := by simp*
+| _ (φ ∧' ψ) m i   := by simp*
+| _ (φ ∨' ψ) m i   := by simp*
+| _ (∀' φ) m i     := by simp*
+| _ (∃' φ) m i     := by simp*
+| _ (pred P) _ _   := by refl
+| _ (papp φ t) m i := by simp[*, term.subst_var0_lift]
 
-@[tls] lemma subst_var0_lift_by_1 {a}  (φ : preformula 𝒮 a)  (i : ℕ) : 
+@[tls] lemma subst_var0_lift_by_1 {a}  (φ : preformula σ a)  (i : ℕ) : 
   (φ ↑ 1 ＠ (i+1))[#0 ⁄ i] = φ := 
 begin
   have h:= subst_var0_lift φ 0 i,
   rwa lift_by_0 at h,
 end
 
-@[tls] lemma subst_var0_for_0_lift_by_1 {a} (φ : preformula 𝒮 a) : 
+@[tls] lemma subst_var0_for_0_lift_by_1 {a} (φ : preformula σ a) : 
   (φ ↑ 1 ＠ 1)[#0 ⁄ 0] = φ := subst_var0_lift_by_1 φ 0
 
-@[simp, tls] lemma subst_for_0_lift_by_1: ∀ {a} ( φ : preformula 𝒮 a) (s : term 𝒮), 
-  (φ ↑ 1 ＠ 0 )[s ⁄ 0] = φ 
-| _ ⊥' _          := by refl
-| _ (t₁ =' t₂) _  := by simp[*, term.subst_for_0_lift_by_1]
-| _ ( φ →' ψ ) _  := by simp[*]
-| _ ( φ ∧' ψ ) _  := by simp[*]
-| _ ( φ ∨' ψ ) _  := by simp[*]
-| _ ( ∀'φ ) s     := begin dsimp, congr, have h:= subst_at_lift φ 0 s (0+1), rw lift_by_0 at h, exact h, end
-| _ ( ∃'φ ) s     := begin dsimp, congr, have h:= subst_at_lift φ 0 s (0+1), rw lift_by_0 at h, exact h, end
-| _ (pred P) _    := by refl
-| _ (papp φ t) _  := by simp[*, term.subst_lift_by_lift]
+@[simp, tls] lemma subst_for_0_lift_by_1: ∀ {a} (φ : preformula σ a) (s : term σ), 
+  (φ ↑ 1 ＠ 0)[s ⁄ 0] = φ 
+| _ ⊥' _         := by refl
+| _ (t₁ =' t₂) _ := by simp[*, term.subst_for_0_lift_by_1]
+| _ (φ →' ψ) _   := by simp[*]
+| _ (φ ∧' ψ) _   := by simp[*]
+| _ (φ ∨' ψ) _   := by simp[*]
+| _ (∀'φ) s      := begin dsimp, congr, have h:= subst_at_lift φ 0 s (0+1), rw lift_by_0 at h, exact h, end
+| _ (∃'φ) s      := begin dsimp, congr, have h:= subst_at_lift φ 0 s (0+1), rw lift_by_0 at h, exact h, end
+| _ (pred P) _   := by refl
+| _ (papp φ t) _ := by simp[*, term.subst_lift_by_lift]
 
-/- If `φ` is a fixpoint for lifting at `i`, then its a fixpoint for lifting at `j` for all `i≤j`  -/
-lemma trivial_lift_monotone {a} {φ : preformula 𝒮 a} {i j} 
+lemma subst_subst : ∀ {a} (φ : preformula σ a) (s₁) {k₁} (s₂) {k₂} (H : k₁ ≤ k₂), 
+    φ [ s₁ ⁄ k₁] [ s₂ ⁄ k₂] = φ [ s₂ ⁄ k₂ + 1] [ (s₁ [s₂ ⁄ k₂ - k₁]) ⁄ k₁ ] 
+| _ ⊥' _ _ _ _ _         := by refl
+| _ (t₁ =' t₂) _ _ _ _ _ := by simp[*, term.subst_subst]
+| _ (φ →' ψ) _ _ _ _ _   := by simp[*]
+| _ (φ ∧' ψ) _ _ _ _ _   := by simp[*]
+| _ (φ ∨' ψ) _ _ _ _ _   := by simp[*]
+| _ (∀' φ) _ _ _ _ _     := by simp[*, add_right_comm]
+| _ (∃' φ) _ _ _ _ _     := by simp[*, add_right_comm]
+| _ (pred P) _ _ _ _ _   := by refl
+| _ (papp φ t) _ _ _ _ _ := by simp[*, term.subst_subst]
+
+
+/- If `φ` is a fixed point for lifting at `i`, then its a fixed point for lifting at `j` for all `i≤j`  -/
+lemma lift_fixed_points_monotone {a} {φ : preformula σ a} {i j} 
   (H : φ ↑ 1 ＠ i = φ) (h : i ≤ j) : φ ↑ 1 ＠ j = φ :=
 begin
   induction j with j,
@@ -693,6 +592,11 @@ begin
       rw [←H, ←lift_lift φ 1 1 h₁, h₂], }, },
 end 
 
+-- We can give improve this lemma a  bit:
+-- - we can state this for fixed points of lifts by m
+-- - we can state this for fixed points of lifts by m ≥ 1 at i
+--   and conclude they are fixed points of lifts by n at j for j≥i
+-- Note that we do not place any conditions on n.
 
 
 /--
@@ -701,26 +605,26 @@ end
   
   In other words, we add `k` universal quantifier in from of `φ`
 -/
-def alls : ∀ (k:ℕ) (φ: formula 𝒮) , formula 𝒮
+def alls : ∀ (k:ℕ) (φ: formula σ) , formula σ
 | 0     φ   := φ 
-| (k+1) φ   := ∀' (alls k φ )
+| (k+1) φ   := ∀' (alls k φ)
 
 -- lemmas about alls
-lemma all_alls: ∀ (φ: formula 𝒮) (k:ℕ) , ∀' (alls k φ) = alls k (∀'φ) 
+lemma all_alls: ∀ (φ: formula σ) (k:ℕ) , ∀' (alls k φ) = alls k (∀'φ) 
 | φ 0 := by refl
 | φ (k+1) := begin unfold alls, congr' 1, apply all_alls, end
 
-lemma alls_succ (k) (φ : formula 𝒮) : alls (k+1) φ = alls k (∀' φ) := begin rw [alls, all_alls], end
+lemma alls_succ (k) (φ : formula σ) : alls (k+1) φ = alls k (∀' φ) := begin rw [alls, all_alls], end
 
-lemma alls_alls: ∀ (φ: formula 𝒮) (m n:ℕ) , alls n (alls m φ) = alls m (alls n φ)
+lemma alls_alls: ∀ (φ: formula σ) (m n:ℕ) , alls n (alls m φ) = alls m (alls n φ)
 | φ 0 n := by refl
 | φ (m+1) n := begin rw alls, rw ←all_alls _ _, rw alls_alls _ m n, refl, end
 
-lemma alls_lift : ∀  (φ: formula 𝒮) (m i n:ℕ), alls n (φ ↑ m ＠ (i+n)) = (alls n φ) ↑ m ＠ i
+lemma alls_lift : ∀  (φ: formula σ) (m i n:ℕ), alls n (φ ↑ m ＠ (i+n)) = (alls n φ) ↑ m ＠ i
 | φ m i 0 := by refl
 | φ m i (n+1) := begin dsimp[alls], congr, rw ←succ_add_eq_succ_add i n, apply alls_lift,end
 
-lemma alls_at_lift  (φ: formula 𝒮) (m n:ℕ) : alls n (φ ↑ m ＠ n) = (alls n φ) ↑ m ＠ 0 :=
+lemma alls_at_lift  (φ: formula σ) (m n:ℕ) : alls n (φ ↑ m ＠ n) = (alls n φ) ↑ m ＠ 0 :=
 begin 
   let h := alls_lift φ m 0 n, 
   rwa zero_add at h, 
@@ -729,19 +633,19 @@ end
 /--
   `substs k i j φ` is the formula `φ[#(k+i) ⁄ k+j]...[#(1+i) ⁄ 1+j][#i ⁄ j]`.
 -/
-def substs : ∀(k i j: ℕ ) ( φ: formula 𝒮), formula 𝒮
+def substs : ∀(k i j: ℕ) (φ: formula σ), formula σ
 | 0 i j φ  := φ 
 | (k+1) i j φ := substs k i j (φ [#(k+i) ⁄ (k+j)])
 
 -- lemmas about substs
-lemma substs_succ (k i j: ℕ ) (φ : formula 𝒮): substs (k+1) i j φ = (substs k (i+1) (j+1) φ) [ #i ⁄ j] :=
+lemma substs_succ (k i j: ℕ) (φ : formula σ): substs (k+1) i j φ = (substs k (i+1) (j+1) φ) [ #i ⁄ j] :=
 begin
   induction k generalizing φ,
   { simp[substs] },
   { simp[*,substs, succ_add_eq_succ_add] }
 end 
 
-lemma all_substs {k i j}{φ : formula 𝒮} : 
+lemma all_substs {k i j}{φ : formula σ} : 
   ∀'(substs k i (j+1) φ) = substs k i j ∀'φ :=
 begin
   induction k generalizing φ,
@@ -749,54 +653,35 @@ begin
   { simp[*,substs, succ_add_eq_succ_add, add_assoc] }
 end
 
-/-
-  ## Remark
-  In the future we need to be able define 
-    
-    "a formula `φ` with free variables among x₀,...,xₖ"
-
-  in our de Bruijn representation of variables.
-  One possible solution is to say that `φ` has no 
-  `k+1`-free variables by traversing inductive definition,
-  to check if each variable is of not `k+1`-free.
-
-  However, we have already developed a more convenient tool
-  in form of lifting. 
-  If `φ` has no `k+1`-free variables then lifting at `k+1` 
-  does not change the formula.
-  We will see that this serves as an adequate definition
-  for our purposes.
--/
-
 /--
   A formula `φ` is `k`-closed if it has no `k`-free variables,
   i.e. if lifting at `k` does not change the formula.
 -/
-@[simp, reducible] def closed {a} (k : ℕ) ( φ : preformula 𝒮 a) := φ ↑ 1 ＠ k = φ 
+@[simp, reducible] def closed {a} (k : ℕ) (φ : preformula σ a) := φ ↑ 1 ＠ k = φ 
 
 /-- A sentence is a `0`-closed formula, i.e. a formula without free variables. -/
-@[simp, reducible] def sentence (φ : formula 𝒮) := closed 0 φ 
-postfix ` is_sentence'`:max := sentence
+@[simp, reducible] def sentence (φ : formula σ) := closed 0 φ 
+postfix ` is_sentence`:max := sentence
 
--- various lemmas involving lifts and substitutions of closed formulas
+/- Various lemmas involving lifts and substitutions of closed formulas -/
 
-lemma closed_all {φ : formula 𝒮} {k} (H : closed (k+1) φ) : closed k (∀' φ) :=
+lemma closed_all {φ : formula σ} {k} (H : closed (k+1) φ) : closed k (∀' φ) :=
 begin dsimp, congr, exact H, end
 
-lemma closed_ex  {φ : formula 𝒮} {k} (H : closed (k+1) φ) : closed k (∃' φ) :=
+lemma closed_ex {φ : formula σ} {k} (H : closed (k+1) φ) : closed k (∃' φ) :=
 begin dsimp, congr, exact H end
 
-lemma lift_closed_id_h { φ : formula 𝒮} {k} (H : closed k φ) (m i) : 
+lemma lift_closed_id_h { φ : formula σ} {k} (H : closed k φ) (m i) : 
   φ ↑ m ＠ (k+i) = φ :=
 begin
   induction m generalizing φ,
   { apply lift_by_0, },
-  { rw [succ_eq_add_one, ←lift_lift_merge φ 1 (le_refl _ ) (le.intro rfl), m_ih H],
-    apply trivial_lift_monotone H (le.intro rfl) },
+  { rw [succ_eq_add_one, ←lift_lift_merge φ 1 (le_refl _) (le.intro rfl), m_ih H],
+    apply lift_fixed_points_monotone H (le.intro rfl) },
 end
 
--- `k`-closed formulas are fixpoints for lifts at reference depth `≥k`
-lemma lift_closed_id { φ : formula 𝒮} {k} (H : closed k φ) (m) {l} (h : k ≤ l): 
+-- `k`-closed formulas are fixed points for lifts at reference depth `≥k`
+lemma lift_closed_id { φ : formula σ} {k} (H : closed k φ) (m) {l} (h : k ≤ l): 
   (φ ↑ m ＠ l) = φ :=
 begin
   cases le_iff_exists_add.mp h with i h_i,
@@ -804,12 +689,12 @@ begin
   exact lift_closed_id_h H m i,
 end
 
--- sentences are fixpoints of all lifts 
-lemma lift_sentence_id {φ : formula 𝒮} (H: sentence φ) { m i } : 
+-- sentences are fixed points of all lifts 
+lemma lift_sentence_id {φ : formula σ} (H: sentence φ) { m i } : 
   (φ ↑ m ＠ i) = φ := lift_closed_id H m (i.zero_le)
 
-lemma lift_set_of_sentences_id {Γ : set $ formula 𝒮} (H : ∀ ϕ ∈ Γ, sentence ϕ) {m i} 
-  : (λ ϕ: formula 𝒮, ϕ ↑ m ＠ i) '' Γ = Γ :=
+lemma lift_set_of_sentences_id {Γ : set $ formula σ} (H : ∀ ϕ ∈ Γ, sentence ϕ) {m i} 
+  : (λ ϕ: formula σ, ϕ ↑ m ＠ i) '' Γ = Γ :=
 begin
   apply ext, intro x,
   apply iff.intro,
@@ -821,26 +706,26 @@ begin
   { intro h, rw mem_image_eq, use x, exact ⟨h, lift_sentence_id (H x h)⟩, },
 end
 
-
-lemma subst_closed_id_h { φ : formula 𝒮} (t:term 𝒮) {k} (i) ( H : closed k φ) : 
+lemma subst_closed_id_h { φ : formula σ} (t:term σ) {k} (i) (H : closed k φ) : 
   (φ [t ⁄ k+i]) = φ :=
 begin
   have h := subst_at_lift φ 0 t (k+i),
   repeat {rwa lift_closed_id_h H _ _ at h,},
 end
 
--- `k`-closed formulas are fixpoints for substitutions at reference depth `≥k`
-lemma subst_closed_id {φ : formula 𝒮}{i}  (H : closed i φ)  (t:term 𝒮) {k} (h : i≤k) : (φ [t ⁄ k]) = φ :=
+-- `k`-closed formulas are fixed points for substitutions at reference depth `≥k`
+lemma subst_closed_id {φ : formula σ}{i}  (H : closed i φ)  (t:term σ) {k} (h : i≤k) : 
+  (φ [t ⁄ k]) = φ :=
 begin
   cases le_iff_exists_add.mp h with j h_j,
   subst h_j, exact subst_closed_id_h t j H,
 end
 
-lemma subst_sentence_id { φ : formula 𝒮} ( H : sentence φ )  {t: term 𝒮} {k:ℕ} :  (φ [t ⁄ k]) = φ 
+lemma subst_sentence_id { φ : formula σ} (H : sentence φ)  {t: term σ} {k:ℕ} :  (φ [t ⁄ k]) = φ 
   := subst_closed_id H t (k.zero_le)
 
-lemma subst_set_of_sentences_id {Γ : set $ formula 𝒮} {t k} (H : ∀f ∈ Γ, sentence f)
-  : (λ (ϕ: formula 𝒮), ϕ[t ⁄ k]) '' Γ = Γ :=
+lemma subst_set_of_sentences_id {Γ : set $ formula σ} {t k} (H : ∀f ∈ Γ, sentence f) : 
+  (λ (ϕ: formula σ), ϕ[t ⁄ k]) '' Γ = Γ :=
 begin
   apply ext, intro x,
   apply iff.intro,
@@ -857,51 +742,49 @@ end
 
   If equal to `0` the formula has no free variables.
 -/
-def max_free_var :  ∀ {a} (φ: preformula 𝒮 a), ℕ 
-| _ ⊥'           := 0
-| _ (t₁ =' t₂)   := max (term.max_free_var t₁) ( term.max_free_var t₂)
-| _ ( ∀'φ )      := (max_free_var φ) - 1
-| _ ( ∃'φ )      := (max_free_var φ) - 1
-| _ ( φ →' ψ )   := max (max_free_var φ) ( max_free_var ψ )
-| _ ( φ ∧' ψ )   := max (max_free_var φ) ( max_free_var ψ )
-| _ ( φ ∨' ψ )   := max (max_free_var φ) ( max_free_var ψ )
-| _ (pred P)     := 0
-| _ (papp φ t)   := max (max_free_var φ) ( term.max_free_var t )
+def max_free_var :  ∀ {a} (φ: preformula σ a), ℕ 
+| _ ⊥'         := 0
+| _ (t₁ =' t₂) := max (term.max_free_var t₁) (term.max_free_var t₂)
+| _ (∀'φ)      := (max_free_var φ) - 1
+| _ (∃'φ)      := (max_free_var φ) - 1
+| _ (φ →' ψ)   := max (max_free_var φ) (max_free_var ψ)
+| _ (φ ∧' ψ)   := max (max_free_var φ) (max_free_var ψ)
+| _ (φ ∨' ψ)   := max (max_free_var φ) (max_free_var ψ)
+| _ (pred P)   := 0
+| _ (papp φ t) := max (max_free_var φ) (term.max_free_var t)
 
 /- This lemma shows that our definition of closed is exactly what our intuition tells us. -/
-lemma closed_max_free_var {a} (φ : preformula 𝒮 a) : closed (max_free_var φ) φ :=
+lemma closed_max_free_var {a} (φ : preformula σ a) : closed (max_free_var φ) φ :=
 begin
   unfold closed,
   induction φ,
   { refl },
-  { have h₁ := term.trivial_lift_monotone (le_max_left (term.max_free_var φ_t)  (term.max_free_var φ_s)) (term.lift_at_max_free_var φ_t),
-    have h₂ := term.trivial_lift_monotone (le_max_right (term.max_free_var φ_t) (term.max_free_var φ_s)) (term.lift_at_max_free_var φ_s),
+  { have h₁ := term.lift_fixed_points_monotone (le_max_left (term.max_free_var φ_t)  (term.max_free_var φ_s)) (term.lift_at_max_free_var φ_t),
+    have h₂ := term.lift_fixed_points_monotone (le_max_right (term.max_free_var φ_t) (term.max_free_var φ_s)) (term.lift_at_max_free_var φ_s),
     rw[max_free_var, formula.lift, h₁,h₂] },
-  { have h₁:= trivial_lift_monotone φ_ih_φ (le_max_left  (max_free_var φ_φ) (max_free_var φ_ψ)),
-    have h₂:= trivial_lift_monotone φ_ih_ψ (le_max_right (max_free_var φ_φ) (max_free_var φ_ψ)),
+  { have h₁:= lift_fixed_points_monotone φ_ih_φ (le_max_left  (max_free_var φ_φ) (max_free_var φ_ψ)),
+    have h₂:= lift_fixed_points_monotone φ_ih_ψ (le_max_right (max_free_var φ_φ) (max_free_var φ_ψ)),
     rw[max_free_var, formula.lift, h₁,h₂] },
-  { have h₁:= trivial_lift_monotone φ_ih_φ (le_max_left  (max_free_var φ_φ) (max_free_var φ_ψ)),
-    have h₂:= trivial_lift_monotone φ_ih_ψ (le_max_right (max_free_var φ_φ) (max_free_var φ_ψ)),
+  { have h₁:= lift_fixed_points_monotone φ_ih_φ (le_max_left  (max_free_var φ_φ) (max_free_var φ_ψ)),
+    have h₂:= lift_fixed_points_monotone φ_ih_ψ (le_max_right (max_free_var φ_φ) (max_free_var φ_ψ)),
     rw[max_free_var, formula.lift, h₁,h₂] },
-  { have h₁:= trivial_lift_monotone φ_ih_φ (le_max_left  (max_free_var φ_φ) (max_free_var φ_ψ)),
-    have h₂:= trivial_lift_monotone φ_ih_ψ (le_max_right (max_free_var φ_φ) (max_free_var φ_ψ)),
+  { have h₁:= lift_fixed_points_monotone φ_ih_φ (le_max_left  (max_free_var φ_φ) (max_free_var φ_ψ)),
+    have h₂:= lift_fixed_points_monotone φ_ih_ψ (le_max_right (max_free_var φ_φ) (max_free_var φ_ψ)),
     rw[max_free_var, formula.lift, h₁,h₂] },
-  { have h := trivial_lift_monotone φ_ih (nat.le_sub_add (max_free_var φ_φ) 1),
+  { have h := lift_fixed_points_monotone φ_ih (nat.le_sub_add (max_free_var φ_φ) 1),
     rw[formula.lift, max_free_var, h], },
-  { have h := trivial_lift_monotone φ_ih (nat.le_sub_add (max_free_var φ_φ) 1),
+  { have h := lift_fixed_points_monotone φ_ih (nat.le_sub_add (max_free_var φ_φ) 1),
     rw[formula.lift, max_free_var, h] },
   { refl },
-  { have h₁:= trivial_lift_monotone φ_ih (le_max_left (max_free_var φ_φ) (term.max_free_var φ_t)),
-    have h₂:= term.trivial_lift_monotone (le_max_right (max_free_var φ_φ) (term.max_free_var φ_t)) (term.lift_at_max_free_var φ_t) ,
+  { have h₁:= lift_fixed_points_monotone φ_ih (le_max_left (max_free_var φ_φ) (term.max_free_var φ_t)),
+    have h₂:= term.lift_fixed_points_monotone (le_max_right (max_free_var φ_φ) (term.max_free_var φ_t)) (term.lift_at_max_free_var φ_t) ,
     rw[max_free_var, formula.lift, h₁, h₂] }
 end 
 
-/--
-  The (universal) closure of a `k`-closed formula, binding its free variables.
--/
-@[reducible] def closure (φ: formula 𝒮) {k} (H: closed k φ) := alls k φ
+/-- The (universal) closure of a `k`-closed formula, binding up to the `k`-th free variable -/
+@[reducible] def closure (φ : formula σ) {k} (H: closed k φ) := alls k φ
 
-lemma closure_is_sentence  { φ : formula 𝒮} {k} (H : closed k φ) : (closure φ H) is_sentence' :=
+lemma closure_is_sentence  {φ : formula σ} {k} (H : closed k φ) : (closure φ H) is_sentence :=
 begin
   induction k generalizing φ,
   { exact H, },
@@ -910,14 +793,19 @@ begin
     exact k_ih (closed_all H), },
 end
 
-lemma lambda_lift_subst_formula {a} {s: term 𝒮} { m i k : ℕ } (h': i ≤ k) 
-  : (λ (ϕ: preformula 𝒮 a), lift (subst ϕ s k) m i) = (λ ϕ, subst ( lift ϕ m i) s (k+m)) :=
-begin funext, apply lift_subst, assumption, end
+def not_free (k) (φ : formula σ) : Prop := ∃ϕ, φ = ϕ ↑ 1 ＠ k
+
+lemma not_free_trival_witness (k)  (φ : formula σ) (h : not_free k φ) : φ = φ[#0 ⁄ k] ↑ 1 ＠ k :=
+begin
+  cases h with ψ ψ_h,
+  subst ψ_h,
+  rw [subst_at_lift, lift_by_0],
+end 
 
 -- /-- Lift operation on sets of formulas. -/
--- @[simp] def lift_set (Γ : set $ formula 𝒮) (m i) : set $ formula 𝒮 := ((λ (ϕ : formula 𝒮), ϕ ↑ m ＠ i) '' Γ)
+-- @[simp] def lift_set (Γ : set $ formula σ) (m i) : set $ formula σ := ((λ (ϕ : formula σ), ϕ ↑ m ＠ i) '' Γ)
 -- /-- Substitution operation on sets of formulas. -/
--- @[simp] def subst_set  (Γ : set $ formula 𝒮) (s k) : set $ formula 𝒮 := ((λ (ϕ : formula 𝒮), ϕ [s ⁄ k]) '' Γ)
+-- @[simp] def subst_set  (Γ : set $ formula σ) (s k) : set $ formula σ := ((λ (ϕ : formula σ), ϕ [s ⁄ k]) '' Γ)
 
 end formula
 
@@ -930,7 +818,7 @@ export formula
 /-!### Proof terms of natural deduction -/
 section proof_terms
 
-local notation φ :: Γ := insert φ Γ 
+local notation φ >> Γ := insert φ Γ 
 
 /--
   An intuitionistic natural deduction proof calculus 
@@ -939,121 +827,51 @@ local notation φ :: Γ := insert φ Γ
   Fresh variables for universal quantifier introduction and existential quantifier elimination
   are introduced by lifting. 
 -/
-
-inductive proof : (set $ formula 𝒮) → formula 𝒮 → Type u
-| hypI {Γ} {φ} (h : φ ∈ Γ) : proof Γ φ 
-| botE {Γ} {φ} (H : proof Γ  ⊥' ) : proof Γ φ
+inductive proof_term : (set $ formula σ) → formula σ → Type u
+| hypI {Γ} {φ} (h : φ ∈ Γ) : proof_term Γ φ 
+| botE {Γ} {φ} (H : proof_term Γ  ⊥') : proof_term Γ φ
 -- implication
-| impI  {Γ} {φ ψ}   (H : proof (φ::Γ) ψ) : proof Γ (φ →' ψ)
-| impE  {Γ} (φ) {ψ} (H₁ : proof Γ φ) (H₂ : proof Γ (φ →' ψ)) : proof Γ ψ
+| impI {Γ} {φ ψ}   (H : proof_term (φ>>Γ) ψ) : proof_term Γ (φ →' ψ)
+| impE {Γ} (φ) {ψ} (H₁ : proof_term Γ φ) (H₂ : proof_term Γ (φ →' ψ)) : proof_term Γ ψ
 -- conjunction
-| andI  {Γ} {φ ψ} (H₁ : proof Γ φ) 
-                  (H₂ : proof Γ ψ) : proof Γ (φ ∧' ψ) 
-| andE₁ {Γ} {φ} (ψ) (H : proof Γ (φ ∧' ψ)) : proof Γ φ
-| andE₂ {Γ} (φ) {ψ} (H : proof Γ (φ ∧' ψ)) : proof Γ ψ
+| andI  {Γ} {φ ψ} (H₁ : proof_term Γ φ) 
+                  (H₂ : proof_term Γ ψ) : proof_term Γ (φ ∧' ψ) 
+| andE₁ {Γ} {φ} (ψ) (H : proof_term Γ (φ ∧' ψ)) : proof_term Γ φ
+| andE₂ {Γ} (φ) {ψ} (H : proof_term Γ (φ ∧' ψ)) : proof_term Γ ψ
 -- disjunction
-| orI₁ {Γ} {φ ψ} (H : proof Γ φ) : proof Γ (φ ∨' ψ)
-| orI₂ {Γ} {φ ψ} (H : proof Γ ψ) : proof Γ (φ ∨' ψ)
-| orE  {Γ}  (φ ψ) {χ} (H  : proof Γ (φ ∨' ψ))  
-                      (H₁ : proof (φ :: Γ) χ) 
-                      (H₂ : proof (ψ :: Γ) χ) : proof Γ χ
+| orI₁ {Γ} {φ ψ} (H : proof_term Γ φ) : proof_term Γ (φ ∨' ψ)
+| orI₂ {Γ} {φ ψ} (H : proof_term Γ ψ) : proof_term Γ (φ ∨' ψ)
+| orE  {Γ}  (φ ψ) {χ} (H  : proof_term Γ (φ ∨' ψ))  
+                      (H₁ : proof_term (φ >> Γ) χ) 
+                      (H₂ : proof_term (ψ >> Γ) χ) : proof_term Γ χ
 -- quantification
-| allI  {Γ} {φ} (H : proof ((λ ϕ, ϕ ↑ 1 ＠ 0) '' Γ) φ) : proof Γ (∀'φ)
-| allE  {Γ} (φ) {t} (H : proof Γ (∀'φ)) : proof Γ (φ [t ⁄ 0])
-| exI   {Γ φ} (t) (H : proof Γ (φ[t ⁄ 0])) : proof Γ  (∃'φ)
-| exE   {Γ ψ} (φ) (H₁ : proof Γ (∃'φ) ) 
-  (H₂ : proof  (φ :: (λ ϕ, ϕ ↑ 1 ＠ 0) '' Γ) (ψ ↑ 1 ＠ 0)) : proof Γ ψ
+| allI  {Γ} {φ} (H : proof_term ((λ ϕ, ϕ ↑ 1 ＠ 0) '' Γ) φ) : proof_term Γ (∀'φ)
+| allE  {Γ} (φ) {t} (H : proof_term Γ (∀'φ)) : proof_term Γ (φ [t ⁄ 0])
+| exI   {Γ φ} (t) (H : proof_term Γ (φ[t ⁄ 0])) : proof_term Γ  (∃'φ)
+| exE   {Γ ψ} (φ) (H₁ : proof_term Γ (∃'φ)) 
+  (H₂ : proof_term  (φ >> (λ ϕ, ϕ ↑ 1 ＠ 0) '' Γ) (ψ ↑ 1 ＠ 0)) : proof_term Γ ψ
 -- equality
-| eqI {Γ} (t) : proof Γ (t =' t)
-| eqE {Γ} {s t φ } (H₁ : proof Γ (s =' t)) (H₂ : proof Γ (φ[s ⁄ 0])) : proof Γ (φ [t ⁄ 0])
-infix ` ⊢ `:55 := proof 
-
-/-
-  The deduction rules for quantifiers deserve some explanation.
- 
-   Γ ⊢ φ[x₀/x] 
-  -------------∀x_I
-    Γ ⊢ ∀x φ 
-
-  with x₀ a variable fresh for Γ.
-
-  Often the context is kept implicit in which case the rule stated as
-
-  ----------- 
-  | x₀      |
-  |   ...   |
-  | φ[x₀/x] |
-  ----------- ∀x_I    x₀ does not occur outside the indicated box
-    Γ ⊢ ∀x φ 
-  
-  In our de Bruijn representation we can introduce a fresh variable  at `0` 
-  by lifting both Γ and ∀φ by `1`. The lower proof term then reads
-
-    `Γ ↑ 1 ＠ 0  ⊢ (∀φ) ↑  1 ＠  0`
-
-  and by definition  
-
-    `(∀φ) ↑  1 ＠  0  = ∀(φ ↑ 1 ＠ 1)`.
-
-  This allows us to apply the above deduction rule for our fresh variable `#0` results in
-
-    `Γ ↑ 1 ＠ 0  ⊢ (φ ↑  1 ＠ 1) [#0 ⁄ 0] `.
-
-  By `subst_var0_for_0_lift_by_1` this simplifies to
-    
-    `Γ ↑ 1 ＠ 0  ⊢ φ`
-
-  and we arrive at our universal introduction.
-
-  Similarly, existential elimination is defined as   
-
-    Γ ⊢ ∃x φ   φ[x₀/x] :: Γ ⊢ ψ      
-    ---------------------------- ∃x_E  
-              Γ ⊢ ψ
-
-  with x₀ a variable fresh for φ, ψ and Γ,
-  or with context kept implicit
-
-            --------------
-            | x₀ φ[x₀/x] |
-            |    ...     |
-    ∃x φ    |     ψ      |      
-    ---------------------- ∃x_E   x₀ does not occur outside the indicated box.
-             ψ
-
-  This time we introduce a fresh variable by lifting `Γ`, `ψ` and `∃φ`. 
-  Again, by definition 
-  
-    `(∃φ) ↑ 1 ＠  0  = ∃(φ ↑  1 ＠ 1)` 
-
-  and to apply the above described deduction rule we need a proof term of the form
-
-   ` (φ ↑  1 ＠ 1) [#0 ⁄ 0] :: (Γ ↑ 1 ＠ 0) ⊢ (ψ ↑ 1 ＠ 0)`
-
-  which by `subst_var0_for_0_lift_by_1`, simplifies to 
-
-    ` φ :: (Γ ↑ 1 ＠ 0) ⊢ (ψ ↑ 1 ＠ 0)`.
-    
-  But this is how we defined existential elimination.
--/
+| eqI {Γ} (t) : proof_term Γ (t =' t)
+| eqE {Γ} {s t φ } (H₁ : proof_term Γ (s =' t)) (H₂ : proof_term Γ (φ[s ⁄ 0])) : proof_term Γ (φ [t ⁄ 0])
+infix ` ⊢ `:55 := proof_term 
 
 /-- 
-  `provable Γ φ` says that there exists a proof of `φ` under the hypotheses in `Γ`,
+  `provable Γ φ` says that there exists a proof_term of `φ` under the hypotheses in `Γ`,
   i.e. it is a fancy way to say that the type `Γ ⊢ φ` is non-empty. 
 -/
-def provable (φ : formula 𝒮) (Γ)  : Prop := nonempty (Γ ⊢ φ)
+def provable (φ : formula σ) (Γ)  : Prop := nonempty (Γ ⊢ φ)
 infix ` is_provable_within `:100 := provable
 
 /--
   The law of excluded middle for when we want to argue in classical logic.
 -/
-def lem : set $ formula 𝒮 := { (φ ∨' ¬'φ) |  (φ: formula 𝒮) (h: φ is_sentence') } -- do we need the extra condition?
+def lem : set $ formula σ := { (φ ∨' ¬'φ) | (φ: formula σ) (h: φ is_sentence) } -- do we need the extra condition?
 
-namespace proof
+namespace proof_term
 /--
-  Rule for weakening the context of a proof by allowing more premises.
+  Rule for weakening the context of a proof_term by allowing more premises.
 -/
-def weak {Δ φ}  (Γ: set $ formula 𝒮 ) ( H : Γ ⊢ φ ) (h: Γ ⊆ Δ): (Δ ⊢ φ) :=
+def weak {Δ φ}  (Γ: set $ formula σ) (H : Γ ⊢ φ) (h: Γ ⊆ Δ): (Δ ⊢ φ) :=
 begin
   induction H generalizing Δ,
   { apply hypI (h H_h) },
@@ -1086,14 +904,14 @@ begin
 end
 
 /--
-  Proof rule for weakening the context of a proof by inserting a single premise.
+  Proof rule for weakening the context of a proof_term by inserting a single premise.
 -/
-def weak1 {Γ} {φ ψ: formula 𝒮} ( H: Γ ⊢ ψ ) :  (φ::Γ) ⊢ ψ := weak Γ H (subset_insert φ Γ)
+def weak1 {Γ} {φ ψ: formula σ} (H: Γ ⊢ ψ) :  (φ>>Γ) ⊢ ψ := weak Γ H (subset_insert φ Γ)
 
 /--
-  Proof rule for weakening the context of a proof from a single premise.
+  Proof rule for weakening the context of a proof_term from a single premise.
 -/
-def weak_singleton {Γ} (φ) {ψ: formula 𝒮} ( H: { φ } ⊢ ψ ) (h: φ ∈ Γ ) :  Γ ⊢ ψ :=
+def weak_singleton {Γ} (φ) {ψ: formula σ} (H: { φ } ⊢ ψ) (h: φ ∈ Γ) :  Γ ⊢ ψ :=
 begin
   apply weak {φ} H,
   assume x xh,
@@ -1103,20 +921,20 @@ begin
 end
 
 -- QoL rules for hypothesis
-def hypI1 {Γ} (φ: formula 𝒮)  : (φ :: Γ ) ⊢ φ := hypI (mem_insert φ Γ)
+def hypI1 {Γ} (φ: formula σ)  : (φ >> Γ) ⊢ φ := hypI (mem_insert φ Γ)
 
-def hypI2 {Γ} (φ ψ: formula 𝒮)  : (φ :: ψ :: Γ ) ⊢ ψ := 
+def hypI2 {Γ} (φ ψ: formula σ)  : φ >> (ψ >> Γ) ⊢ ψ := 
 begin
   apply hypI, right, exact mem_insert ψ Γ,
 end
 /--
   Rule for top introduction.
 -/
-def topI {Γ: set $ formula 𝒮} : Γ ⊢ ⊤' := begin apply impI, apply hypI1, end
+def topI {Γ: set $ formula σ} : Γ ⊢ ⊤' := begin apply impI, apply hypI1, end
 
 
 -- rules for implications
-def impE_insert {Γ} {φ ψ: formula 𝒮} (H₁ : Γ ⊢ (φ →' ψ )) : φ :: Γ ⊢ ψ  :=
+def impE_insert {Γ} {φ ψ: formula σ} (H₁ : Γ ⊢ (φ →' ψ)) : φ >> Γ ⊢ ψ  :=
 begin
   apply impE φ, 
   apply hypI1, 
@@ -1127,7 +945,7 @@ end
 /--
   Proof rule for reflexivity of implications.
 -/
-def impI_refl {Γ} (φ : formula 𝒮) : Γ ⊢ (φ →' φ) := 
+def impI_refl {Γ} (φ : formula σ) : Γ ⊢ (φ →' φ) := 
 begin
     apply impI, apply hypI1,
 end
@@ -1135,7 +953,7 @@ end
 /--
   Proof rule for transitivity of implications.
 -/
-def impI_trans  {Γ} (φ ψ χ : formula 𝒮) (H₁: Γ ⊢ (φ →' ψ )) (H₂ : Γ ⊢ (ψ  →' χ )) : Γ ⊢ (φ  →' χ) :=
+def impI_trans  {Γ} (φ ψ χ : formula σ) (H₁: Γ ⊢ (φ →' ψ)) (H₂ : Γ ⊢ (ψ  →' χ)) : Γ ⊢ (φ  →' χ) :=
 begin
   apply impI, 
   apply impE ψ, 
@@ -1144,53 +962,52 @@ begin
 end
 
 /--
-  QoL proof rule for universal quantification elimination.
+  QoL proof_term rule for universal quantification elimination.
 -/
-def allE' {Γ} (φ) (t: term 𝒮) {ψ}  (H : Γ ⊢ (∀'φ)) (h: ψ  = φ[t ⁄ 0]) : Γ ⊢ ψ :=
+def allE' {Γ} (φ) (t: term σ) {ψ}  (H : Γ ⊢ (∀'φ)) (h: ψ  = φ[t ⁄ 0]) : Γ ⊢ ψ :=
 begin subst h, apply allE, assumption, end
 
 /--
   Proof rule for a common case of universal quantification elimination.
 -/
-def allE_var0 {Γ} {φ: formula 𝒮}  (H : Γ ⊢ (∀'φ) ↑ 1 ＠ 0) : Γ ⊢ φ  :=
+def allE_var0 {Γ} {φ: formula σ}  (H : Γ ⊢ (∀'φ) ↑ 1 ＠ 0) : Γ ⊢ φ  :=
 begin
-  apply allE' (φ ↑ 1 ＠  1) #0,
+  apply allE' (φ ↑ 1 ＠ 1) #0,
   { exact H, }, 
   { symmetry, exact subst_var0_lift_by_1 φ 0, } 
 end
 
-
 /--
   Proof rule for equality elimination. _(QoL)_
 -/
-def eqE' {Γ} {ψ}  (s t) (φ : formula 𝒮) (H₁ : Γ ⊢ (s =' t)) (H₂ : Γ ⊢ (φ [s ⁄ 0])) (h:  ψ = φ[t ⁄ 0]) : Γ ⊢ ψ :=
+def eqE' {Γ} {ψ}  (s t) (φ : formula σ) (H₁ : Γ ⊢ (s =' t)) (H₂ : Γ ⊢ (φ [s ⁄ 0])) (h:  ψ = φ[t ⁄ 0]) : Γ ⊢ ψ :=
 begin rw h, apply eqE H₁ H₂, end
 
 /-- Proof rule for congruence introduction. -/
-def congrI {Γ} {t s₁ s₂: term 𝒮} (H :  Γ ⊢ (s₁ =' s₂)) :  Γ ⊢ ( t[s₁ ⁄ 0] =' t[s₂ ⁄ 0] ):=
+def congrI {Γ} {t s₁ s₂: term σ} (H :  Γ ⊢ (s₁ =' s₂)) :  Γ ⊢ (t[s₁ ⁄ 0] =' t[s₂ ⁄ 0]):=
 begin
-  apply eqE' s₁ s₂ (( (t[s₁⁄ 0] ↑ 1 ＠ 0 )=' t)) H;
+  apply eqE' s₁ s₂ (((t[s₁⁄ 0] ↑ 1 ＠ 0)=' t)) H;
   rw [subst, term.subst_for_0_lift_by_1 (term.subst t _ 0) _],
   apply eqI,
 end
 
 /-- Proof rule for congruence introduction. -/
-def congrI' {Γ} {t₁ s₁ t₂ s₂ : term 𝒮} (t) (H: Γ ⊢ s₁ =' s₂) 
+def congrI' {Γ} {t₁ s₁ t₂ s₂ : term σ} (t) (H: Γ ⊢ s₁ =' s₂) 
   (h₁: t₁ = t[s₁ ⁄ 0]) (h₂: t₂ = t[s₂ ⁄ 0]) : Γ ⊢ (t₁ =' t₂) := 
 begin rw [h₁, h₂], apply congrI H, end
 
 /-- Proof rule for reflexivity of equality. -/
-def eqI_refl {Γ} (t: term 𝒮): Γ ⊢ (t =' t) := @eqI 𝒮 Γ t
+def eqI_refl {Γ} (t: term σ): Γ ⊢ (t =' t) := @eqI σ Γ t
 
 /-- Proof rule for symmetry of equality. -/
-def eqI_symm {Γ} (s t : term 𝒮) (H : Γ ⊢ (s =' t)) : Γ ⊢ (t =' s) :=
+def eqI_symm {Γ} (s t : term σ) (H : Γ ⊢ (s =' t)) : Γ ⊢ (t =' s) :=
 begin
   apply eqE' s t (#0 =' (s ↑ 1 ＠ 0)) H;
   rw [subst, term.subst_var0, term.subst_for_0_lift_by_1],
   apply eqI, 
 end
 /-- Proof rule for transitivity of equality. -/
-def eqI_trans {Γ} ( s t u : term 𝒮) (H₁ : Γ ⊢ (s =' t) ) (H₂ : Γ ⊢ (t =' u)) : proof Γ ( s =' u) :=
+def eqI_trans {Γ} (s t u : term σ) (H₁ : Γ ⊢ (s =' t)) (H₂ : Γ ⊢ (t =' u)) : proof_term Γ (s =' u) :=
 begin
   apply eqE' t u ((s ↑ 1 ＠ 0) =' #0) H₂;
   rw[subst, term.subst_for_0_lift_by_1, term.subst_var0], 
@@ -1200,17 +1017,17 @@ end
 /- biconditionals -/
 
 /-- Proof rule for introducing a biconditional. -/
-def iffI {Γ} {φ ψ : formula 𝒮} (H₁ : Γ ⊢ φ →' ψ) (H₂ : Γ ⊢ ψ →' φ)  : Γ ⊢ (φ  ↔' ψ) :=
+def iffI {Γ} {φ ψ : formula σ} (H₁ : Γ ⊢ φ →' ψ) (H₂ : Γ ⊢ ψ →' φ)  : Γ ⊢ (φ  ↔' ψ) :=
 begin apply andI; assumption, end
 
-def iffE_r {Γ} {φ ψ : formula 𝒮} (H : Γ ⊢ φ ↔' ψ)  : (Γ ⊢ φ →' ψ) := andE₁ _ H
+def iffE_r {Γ} {φ ψ : formula σ} (H : Γ ⊢ φ ↔' ψ)  : (Γ ⊢ φ →' ψ) := andE₁ _ H
 
-def iffE_l {Γ} {φ ψ : formula 𝒮} (H : Γ ⊢ φ ↔' ψ)  : (Γ ⊢ ψ →' φ) := andE₂ _ H
+def iffE_l {Γ} {φ ψ : formula σ} (H : Γ ⊢ φ ↔' ψ)  : (Γ ⊢ ψ →' φ) := andE₂ _ H
 
 /--
   Proof rule for eliminating the right part of a biconditional.
 -/
-def iffE₁ {Γ} {φ: formula 𝒮} (ψ : formula 𝒮) (H₁ : Γ ⊢ ψ) (H₂ : Γ ⊢ φ ↔' ψ)  : Γ ⊢ φ :=
+def iffE₁ {Γ} {φ: formula σ} (ψ : formula σ) (H₁ : Γ ⊢ ψ) (H₂ : Γ ⊢ φ ↔' ψ)  : Γ ⊢ φ :=
 begin
   apply impE ψ,
   { exact H₁, },
@@ -1218,7 +1035,7 @@ begin
 end
 
 /-- Proof rule for eliminating the left part of a biconditional. -/
-def iffE₂ {Γ} (φ) {ψ : formula 𝒮} (H₁ : Γ ⊢ φ) (H₂ : Γ ⊢ φ ↔' ψ)  : (Γ ⊢  ψ) :=
+def iffE₂ {Γ} (φ) {ψ : formula σ} (H₁ : Γ ⊢ φ) (H₂ : Γ ⊢ φ ↔' ψ)  : (Γ ⊢  ψ) :=
 begin
   apply impE φ,
   { exact H₁, },
@@ -1226,10 +1043,10 @@ begin
 end
 
 /-- Proof rule for reflexivity of biconditionals.-/
-def iffI_refl {Γ} (φ : formula 𝒮) : Γ ⊢ (φ ↔' φ) := begin apply iffI; apply impI_refl,end
+def iffI_refl {Γ} (φ : formula σ) : Γ ⊢ (φ ↔' φ) := begin apply iffI; apply impI_refl,end
 
 /-- Proof rule for transitivity of biconditionals. -/
-def iffI_trans {Γ} {φ} (ψ: formula 𝒮) {χ}  (H₁: Γ ⊢ (φ ↔' ψ)) (H₂ : Γ ⊢ (ψ ↔' χ)) : Γ ⊢ (φ ↔' χ) :=
+def iffI_trans {Γ} {φ} (ψ: formula σ) {χ}  (H₁: Γ ⊢ (φ ↔' ψ)) (H₂ : Γ ⊢ (ψ ↔' χ)) : Γ ⊢ (φ ↔' χ) :=
 begin
     apply andI;
     apply impI_trans _ ψ _,
@@ -1238,18 +1055,18 @@ begin
 end
 
 /-- Proof rule for symmetry of biconditionals. -/
-def iffI_symm {Γ} {φ ψ: formula 𝒮}  (H: Γ ⊢ (φ ↔' ψ)) : Γ ⊢ (ψ ↔' φ) := 
+def iffI_symm {Γ} {φ ψ: formula σ}  (H: Γ ⊢ (φ ↔' ψ)) : Γ ⊢ (ψ ↔' φ) := 
 begin apply iffI, apply andE₂, exact H, apply andE₁, exact H, end
 
 
-/-- Proof rule for substiuting a term for free variable. -/
-def substI {Γ} {φ : formula 𝒮} (t k) (H: Γ ⊢ φ ) : (λ ϕ, ϕ[t ⁄ k])'' Γ ⊢ φ[t ⁄ k] :=
+/-- Proof rule for substituting a term for free variable. -/
+def substI {Γ} {φ : formula σ} (t k) (H: Γ ⊢ φ) : (λ ϕ, ϕ[t ⁄ k])'' Γ ⊢ φ[t ⁄ k] :=
 begin
   induction H generalizing k,
-  { apply hypI, exact mem_image_of_mem (λ (ϕ : preformula 𝒮 0), ϕ [t ⁄ k]) H_h, },
+  { apply hypI, exact mem_image_of_mem (λ (ϕ : preformula σ 0), ϕ [t ⁄ k]) H_h, },
   { apply botE, apply H_ih, },
 
-  { apply impI, rw ← (@image_insert_eq _ _ (λ (x : preformula 𝒮 0), x[t ⁄ k])), exact H_ih k, },
+  { apply impI, rw ← (@image_insert_eq _ _ (λ (x : preformula σ 0), x[t ⁄ k])), exact H_ih k, },
   { apply impE (H_φ [t ⁄ k]), exact H_ih_H₁ k, exact H_ih_H₂ k, },
 
   { apply andI, exact H_ih_H₁ k, exact H_ih_H₂ k, },
@@ -1281,15 +1098,16 @@ begin
     exact subst_subst H_φ H_t t (k.zero_le), }
 end
 
-/-- Proof rule for introducing `m` fresh variables at index `i` to a proof. -/
-def liftI {Γ} {φ : formula 𝒮} (m i : ℕ) (H: Γ ⊢ φ) : (λ (ϕ :formula 𝒮), ϕ ↑ m ＠  i ) '' Γ ⊢ (φ ↑ m ＠  i) :=
+/-- Proof rule for introducing `m` fresh variables at `i`. -/
+def liftI {Γ} {φ : formula σ} (m i : ℕ) (H: Γ ⊢ φ) 
+  : (λ (ϕ :formula σ), ϕ ↑ m ＠ i) '' Γ ⊢ (φ ↑ m ＠ i) :=
 begin
   induction H generalizing i,
-  { apply hypI, exact mem_image_of_mem (λ (ϕ : preformula 𝒮 0),  ϕ ↑ m ＠  i) H_h, },
+  { apply hypI, exact mem_image_of_mem (λ (ϕ : preformula σ 0),  ϕ ↑ m ＠ i) H_h, },
   { apply botE, exact H_ih i, },
 
   { apply impI, have:= H_ih i, rwa image_insert_eq at this, },
-  { apply impE (H_φ ↑ m ＠  i) , exact H_ih_H₁ i, exact H_ih_H₂ i,},
+  { apply impE (H_φ ↑ m ＠ i) , exact H_ih_H₁ i, exact H_ih_H₂ i,},
 
   { apply andI, apply H_ih_H₁ i, apply H_ih_H₂ i, },
   { apply andE₁, apply H_ih i, },
@@ -1317,24 +1135,34 @@ begin
   { apply eqE' _ _ _ (H_ih_H₁ i),
     have h₁:= symm (subst0_lift_by_lift H_φ),
     have h₂ := H_ih_H₂ i, rw h₁ at h₂, exact h₂,
-    exact symm ( subst0_lift_by_lift _ ), },
+    exact symm (subst0_lift_by_lift _), },
 end
 
--- rules for dealing with universal closures
-def allsI {Γ} {φ: formula 𝒮}  (n) (H: (λ ϕ , ϕ ↑ n ＠  0) '' Γ ⊢ φ) :  Γ ⊢ alls n φ  :=
+/-- Proof rule for removing a single fresh variables at `0`. -/
+def liftE_h {Γ} {φ : formula σ} (m i : ℕ) (H:  (λ (ϕ :formula σ), ϕ ↑ 1 ＠ 0) '' Γ ⊢ (φ ↑ 1 ＠ 0)) 
+  : Γ ⊢ φ :=
+begin
+  rw ←subst_for_0_lift_by_1 φ #0,
+  apply allE,
+  apply allI,
+  exact H,
+end
+
+/-- Proof rule for binding the first `n` variables with universal quantifiers. -/
+def allsI {Γ} {φ: formula σ}  (n) (H: (λ ϕ , ϕ ↑ n ＠ 0) '' Γ ⊢ φ) :  Γ ⊢ alls n φ  :=
 begin
   induction n generalizing φ Γ,
   { simp [lift_by_0] at H, assumption,},
   { rw[alls], 
     apply allI,
-    have h : (λ (ϕ : preformula 𝒮 0), ϕ ↑ n_n.succ ＠ 0) 
-      = (λ (ϕ : preformula 𝒮 0), ϕ ↑ n_n ＠ 0) ∘ (λ (ϕ : preformula 𝒮 0), ϕ ↑ 1＠ 0),
+    have h : (λ (ϕ : preformula σ 0), ϕ ↑ n_n.succ ＠ 0) 
+      = (λ (ϕ : preformula σ 0), ϕ ↑ n_n ＠ 0) ∘ (λ (ϕ : preformula σ 0), ϕ ↑ 1＠ 0),
     begin funext, dsimp, rw lift_at_lift_merge, rw add_comm 1 n_n, end,
     rw [h, image_comp] at H,
     exact n_ih H, },
 end
-
-def allsE  {Γ} {φ: formula 𝒮}  (n i) (H :  Γ ⊢ (alls n φ)) :  Γ ⊢ substs n i 0 φ :=
+/-- Proof rule unbinding the `n` universal quantifiers. -/
+def allsE  {Γ} {φ: formula σ}  (n i) (H :  Γ ⊢ (alls n φ)) :  Γ ⊢ substs n i 0 φ :=
 begin
   induction n generalizing φ i,
   { exact H,},
@@ -1345,14 +1173,15 @@ begin
     exact n_ih (i+1) H, },
 end
 
-def allsE' {Γ} (n) {φ  : formula 𝒮} (H : Γ ⊢ (alls n φ)) : (λ ϕ , ϕ ↑ n ＠  0) '' Γ ⊢ φ  :=
+/-- Proof rule unbinding the `n` universal quantifiers. -/
+def allsE' {Γ} (n) {φ  : formula σ} (H : Γ ⊢ (alls n φ)) : (λ ϕ , ϕ ↑ n ＠ 0) '' Γ ⊢ φ  :=
 begin
   induction n generalizing φ Γ,
-  { have h :  (λ (ϕ: formula 𝒮) , ϕ ↑ 0 ＠  0) = id, from begin funext, rw lift_by_0, refl, end,
+  { have h :  (λ (ϕ: formula σ) , ϕ ↑ 0 ＠ 0) = id, from begin funext, rw lift_by_0, refl, end,
     rw [h, image_id] at *, 
     rwa alls at H, },
-  { have h: (λ (ϕ : preformula 𝒮 0), ϕ ↑ n_n.succ ＠ 0) 
-          = (λ (ϕ : preformula 𝒮 0), ϕ ↑ 1 ＠ 0) ∘ (λ (ϕ : preformula 𝒮 0), ϕ ↑ n_n ＠ 0),
+  { have h: (λ (ϕ : preformula σ 0), ϕ ↑ n_n.succ ＠ 0) 
+          = (λ (ϕ : preformula σ 0), ϕ ↑ 1 ＠ 0) ∘ (λ (ϕ : preformula σ 0), ϕ ↑ n_n ＠ 0),
     begin funext, dsimp, rw lift_at_lift_merge, end,
     rw [alls_succ] at H,
     apply allE_var0,
@@ -1361,21 +1190,21 @@ begin
     exact n_ih H, },
 end
 
-def modus_tollens {Γ} {φ} (ψ: formula 𝒮) (H₁: Γ ⊢ (φ →' ψ)) (H₂: Γ ⊢ ¬'ψ) : Γ ⊢ ¬'φ  :=
-begin
-  apply impI,
-  apply impE ψ,
-  { apply impE_insert,
-   assumption, },
-  { apply weak1,
-    assumption, },
-end
-end proof
+-- def modus_tollens {Γ} {φ} (ψ: formula σ) (H₁: Γ ⊢ (φ →' ψ)) (H₂: Γ ⊢ ¬'ψ) : Γ ⊢ ¬'φ  :=
+-- begin
+--   apply impI,
+--   apply impE ψ,
+--   { apply impE_insert,
+--    assumption, },
+--   { apply weak1,
+--     assumption, },
+-- end
+end proof_term
 
-export proof
+export proof_term
 
 /-- Formal proof that there always exists an object of discourse. -/
-def let_there_be_light : (∅ : set $ formula 𝒮) ⊢ ∃'(#0 =' #0) :=
+def let_there_be_light : (∅ : set $ formula σ) ⊢ ∃'(#0 =' #0) :=
 begin
   apply exI #0,
   apply eqI,
@@ -1387,26 +1216,26 @@ end
    Therefore, Socrates is mortal." .   
 -/
 
-example {Γ:set $ formula 𝒮}{φ ψ χ}  (H₁: Γ ⊢ ∀'(φ →' ψ))  (H₂: Γ ⊢ ∀'(ψ →' χ)) : Γ ⊢ ∀' (φ →' χ) :=
+example {Γ:set $ formula σ}{φ ψ χ}  (H₁: Γ ⊢ ∀'(φ →' ψ))  (H₂: Γ ⊢ ∀'(ψ →' χ)) : Γ ⊢ ∀' (φ →' χ) :=
 begin
   apply allI,
   apply impI,
   apply impE ψ,
   { apply impE_insert,
-    apply allE' ((φ →' ψ) ↑ 1 ＠  1) #0,
+    apply allE' ((φ →' ψ) ↑ 1 ＠ 1) #0,
     rw ←formula.lift,
     apply liftI,
     exact H₁,
     rw subst_var0_lift_by_1, },
   { apply weak1,
-    apply allE' ((ψ →' χ) ↑ 1 ＠  1) #0,
+    apply allE' ((ψ →' χ) ↑ 1 ＠ 1) #0,
     rw ←formula.lift,
     apply liftI,
     exact H₂,
     rw subst_var0_lift_by_1, },
 end
 
-example {Γ:set $ formula 𝒮}{φ ψ χ}  (H₁: Γ ⊢ ∀'(φ →' ψ) )  (H₂: Γ ⊢ ∀'(ψ →' χ)) : Γ ⊢ ∀' (φ →' χ) :=
+example {Γ:set $ formula σ}{φ ψ χ}  (H₁: Γ ⊢ ∀'(φ →' ψ))  (H₂: Γ ⊢ ∀'(ψ →' χ)) : Γ ⊢ ∀' (φ →' χ) :=
 begin
   apply allI,
   apply impI,
@@ -1415,7 +1244,7 @@ begin
   swap,
   apply weak1,
   all_goals 
-  { apply allE' ( _ ↑ 1 ＠  1) #0,
+  { apply allE' (_ ↑ 1 ＠ 1) #0,
     rw ←formula.lift,
     apply liftI,
     swap,
