src/izf.lean
@@ -7,14 +7,9 @@ import data.set
 In this file we define the signature and axioms of intuitionistic Zermelo-Fraenkel set theory
 and give a natural deduction proof of the induction principle in its set theoretical form.
 
-We also briefly discuss how statements about named variables like 
-  "φ is a formula with B not free"
-in the formulation of the axiom schemes of separation and collection
-can be translated to De Bruijn variables using lifts.
-
 ## Main results
 
-- `omega_smallest_inductive_provable_within_izf`: 
+- `omega_smallest_inductive_provable`: 
     we show that ZFC proves that ω is the smallest inductive set. a direct consequence of
 - `omega_smallest_inductive`: 
     a natural deduction proof that ω is the smallest inductive set
@@ -52,15 +47,15 @@ inductive func_symb : ℕ → Type u
 | pair  : func_symb 2
 --| succ  : func_symb 1
  
-def 𝒮 : signature := { func_symb:= izf.func_symb , pred_symb:= izf.pred_symb }
+def σ : signature := { func_symb:= izf.func_symb , pred_symb:= izf.pred_symb }
 
 -- Definitions and notations for our functions
-@[simp]def emptyset                 : term 𝒮 := (func func_symb.empty : term 𝒮)
-@[simp]def omegaset                 : term 𝒮 := (func func_symb.omega : term 𝒮)
-@[simp]def unionset (t : term 𝒮)    : term 𝒮 :=  fapp (func func_symb.union) t
-@[simp]def powerset (t : term 𝒮)    : term 𝒮 := fapp (func func_symb.power) t
-@[simp]def pairset (t₁ t₂ : term 𝒮) : term 𝒮 := fapp (fapp (func func_symb.pair) t₁) t₂
---def successorset (t: term 𝒮) : term 𝒮 :=  fapp (func func_symb.succ) t
+@[simp]def emptyset                 : term σ := (func func_symb.empty : term σ)
+@[simp]def omegaset                 : term σ := (func func_symb.omega : term σ)
+@[simp]def unionset (t : term σ)    : term σ :=  fapp (func func_symb.union) t
+@[simp]def powerset (t : term σ)    : term σ := fapp (func func_symb.power) t
+@[simp]def pairset (t₁ t₂ : term σ) : term σ := fapp (fapp (func func_symb.pair) t₁) t₂
+--def successorset (t: term σ) : term σ :=  fapp (func func_symb.succ) t
 
 notation `⌀`  := emptyset -- this is not ∅; type ⌀ using \diameter
 notation `ω`  := omegaset
@@ -70,27 +65,31 @@ prefix 𝒫      := powerset
 notation ⦃ a ` , ` b ⦄ := pairset a b  -- type ⦃ and ⦄ using \{{ and \}}
 notation ⦃ a ⦄ := pairset a a
 
--- Definition and notation for our predicate
-@[simp] def memb (t₁ t₂: term 𝒮): formula 𝒮 := papp (papp (pred pred_symb.elem) t₁) t₂
+/-- Definition of the membership predicate.-/
+@[simp] def memb (t₁ t₂: term σ): formula σ := papp (papp (pred pred_symb.elem) t₁) t₂
 infix ` ∈' `:100 := memb
 
 -- Meta predicates and functions
--- def subset (t₁ t₂: term 𝒮): formula 𝒮 := papp (papp (pred_symb pred_symb.subset) t₁) t₂
-@[simp] def subset (t₁ t₂: term 𝒮): formula 𝒮 := ∀'( #0 ∈' (t₁ ↑ 1 ＠  0) →' #0 ∈' (t₂ ↑ 1 ＠  0))
+-- def subset (t₁ t₂: term σ): formula σ := papp (papp (pred_symb pred_symb.subset) t₁) t₂
+/-- Definition of the subset predicate.-/
+@[simp] def subset (t₁ t₂: term σ): formula σ := ∀'(#0 ∈' (t₁ ↑ 1 ＠ 0) →' #0 ∈' (t₂ ↑ 1 ＠ 0))
 infix ` ⊆' `:100 := subset
 
-@[simp] def successor_set (t: term 𝒮) : term 𝒮 := ⋃⦃ t , ⦃ t ⦄ ⦄
+/-- Definition of the successor set.-/
+@[simp] def successor_set (t: term σ) : term σ := ⋃⦃ t , ⦃ t ⦄ ⦄
 prefix `S`:max := successor_set
 
-@[simp] def is_inductive (t : term 𝒮) 
-  := ⌀ ∈' t ∧' ∀' (#0 ∈' (t ↑ 1 ＠  0) →' S #0 ∈' (t ↑ 1 ＠  0))
-postfix ` is_inductive`:max := is_inductive
+/-- Definition of inductive sets.-/
+@[simp] def inductive_def (t : term σ) := 
+  ⌀ ∈' t ∧' ∀' (#0 ∈' (t ↑ 1 ＠ 0) →' S #0 ∈' (t ↑ 1 ＠ 0))
+postfix ` is_inductive`:max := inductive_def
 
-@[simp] def unique_in_var0 (φ: formula 𝒮) : formula 𝒮 
-  :=  ∀' ∀' ((φ ↑ 1 ＠ 1 ) ∧' (φ ↑ 1 ＠ 0) →' (#0 =' #1) )
+/-- Definition of uniqueness in the first variable. -/
+@[simp] def unique_in_var0 (φ: formula σ) : formula σ :=  
+  ∀' ∀' ((φ ↑ 1 ＠ 1) ∧' (φ ↑ 1 ＠ 0) →' (#0 =' #1))
 
-@[simp] def unique_ex (φ : formula 𝒮) : formula 𝒮 
-  := (∃'φ) ∧' (unique_in_var0 φ)
+/-- Definition of the unique existential quantifier. -/
+@[simp] def unique_ex (φ : formula σ) : formula σ := (∃'φ) ∧' (unique_in_var0 φ)
 prefix `∃!`:110 := unique_ex 
 
 end izf_signature
@@ -110,14 +109,14 @@ end izf_signature
 -/
 
 -- this seems helps pretty printing reduced terms and formulas and makes them much easier to read
-notation `'⌀` := func func_symb.empty
-notation `'ω` := func func_symb.omega
-notation `'⋃` t :=  fapp (func func_symb.union) t
-notation `'𝒫` t := fapp (func func_symb.power) t 
---notation `'S` t := fapp (func func_symb.succ) t
-notation `'{ ` a ` , `b` }` := fapp (fapp (func func_symb.pair) a) b
-notation s ` '∈ `:100 t := papp (papp (pred pred_symb.elem) s) t
-notation s ` '⊆ `:100 t := papp (papp (pred pred_symb.subset) s) t
+-- notation `'⌀` := func func_symb.empty
+-- notation `'ω` := func func_symb.omega
+-- notation `'⋃` t :=  fapp (func func_symb.union) t
+-- notation `'𝒫` t := fapp (func func_symb.power) t 
+-- --notation `'S` t := fapp (func func_symb.succ) t
+-- notation `'{ ` a ` , `b` }` := fapp (fapp (func func_symb.pair) a) b
+-- notation s ` '∈ `:100 t := papp (papp (pred pred_symb.elem) s) t
+-- notation s ` '⊆ `:100 t := papp (papp (pred pred_symb.subset) s) t
 
 -- after
 -- #reduce (⌀ ∈' ω  ∧' ⦃ ⌀, S⦃ #3 ⦄ ⦄∈' 𝒫#1) ↑ 1 ＠ 1      
@@ -128,89 +127,55 @@ notation s ` '⊆ `:100 t := papp (papp (pred pred_symb.subset) s) t
 
 section izf_axioms
 
+/- Definitions and lemmas related to the axiom scheme of separation -/
 namespace separation
-/-
-  The separation axiom scheme is defined as the closure* of
-    `∀A ∃B ∀x ( x ∈ B ↔ x ∈ A ∧ φ)` (1)
-  for all formulas `φ` such that `B` is not free in `φ`.
-  Ignoring variable names we see that the existential quantifier 
-  binds variables of `φ` pointing to `1`.
-  We can avoid such bindings by simply requiring that 
-    `φ = ψ ↑ 1 ＠ 1` 
-  for a formula `ψ`.
-  On the other hand, if no index points to `1`, then one can check that
-    `φ = φ[#0/1] ↑ 1 ＠ 1`**,
-  reducing the side condition to a question about lifts.
-  As an added bonus this allows us to state the axiom of separation 
-  without any side condition as the closure of the formula below.
+open fol
 
-  (*) See further below.
-  (**) Exercise 1: Generalize this and proof it in lean.
--/
-@[simp] def formula (φ : formula 𝒮): formula 𝒮 
-  := ∀' ∃' ∀' ((#0 ∈' #1)  ↔' (#0 ∈' #2 ∧' (φ  ↑ 1 ＠  1)))
+/-- Defintion of the axiom scheme of separation with free variables. -/
+@[simp] def free_formula (φ : formula σ): formula σ := 
+  ∀' ∃' ∀' ((#0 ∈' #1)  ↔' (#0 ∈' #2 ∧' (φ ↑ 1 ＠ 1)))
 
-/-
-  To define the closure of (1) we usually state separation in terms of formulas φ(x, A, x₁, ... , xₙ)
-  with free variables among (but not necessarily exactly) x, A, x₁, ... , xₙ.
-  The closure is then given by
-    `∀xₙ ... ∀x₁ ∀A ∃B ∀x ( x ∈ B ↔ x ∈ A ∧ φ)`. (1')
-  For our De Bruijn representation of variables this translates to `φ_h: closed (n+2) φ`,
-  so `formula φ` has no n-free variables (see lemma below) and its closure (as defined in fol)
-  gives us an De Bruijn version of (1') and invariance under lifts.
--/
-lemma closed{k} {φ} (H: closed (k+2) φ) : closed k (formula φ)  :=
+lemma closed{k} {φ} (H: closed (k+2) φ) : closed k (free_formula φ)  :=
 begin
   have h₁: ¬ k + 3 ≤ 2, by linarith,
   have h₂: 1 ≤ k+2, by linarith,
-  have h₃:  φ ↑  1 ＠  1 ↑ 1  ＠ (k + 3) = φ ↑ 1 ＠ 1,
+  have h₃:  φ ↑ 1 ＠ 1 ↑ 1 ＠ (k + 3) = φ ↑ 1 ＠ 1,
     begin  rw ←(lift_lift φ 1 1 h₂), congr, exact H, end,
   simp[h₁, h₃],
 end
 
-def sentence  (φ : fol.formula 𝒮) {n : ℕ} (φ_h: formula.closed (n+2) φ) : fol.formula 𝒮 
-  := formula.closure (formula φ) (closed φ_h)
+/-- Defintion of the axiom scheme of separation. -/
+def formula (φ : fol.formula σ) {n : ℕ} (φ_h: formula.closed (n+2) φ) : fol.formula σ := 
+  formula.closure (free_formula φ) (closed φ_h)
 
-lemma is_sentence {k : ℕ} (φ  : fol.formula 𝒮) (H: fol.formula.closed (k+2) φ) :
-  (sentence φ H) is_sentence' := begin exact closure_is_sentence (closed H) end
+lemma formula_is_sentence {k : ℕ} (φ : fol.formula σ) (H: formula.closed (k+2) φ) :
+  (formula φ H) is_sentence := begin exact closure_is_sentence (closed H) end
 
-lemma lift_sentence (φ) (n) (φ_h: fol.formula.closed (n+2) φ) (m i) 
-  : (sentence φ φ_h) ↑ m ＠  i = sentence φ φ_h := lift_sentence_id (is_sentence _ _)
-
+lemma lift_sentence (φ) (n) (φ_h: fol.formula.closed (n+2) φ) (m i) : 
+  (formula φ φ_h) ↑ m ＠ i = formula φ φ_h := lift_sentence_id (formula_is_sentence _ _)
 
 /- To following definition and lemmas are used to make future proofs more explicit and readable. -/
-lemma mem {Γ:set $ fol.formula 𝒮} (φ) (k) (φ_h: formula.closed (k+2) φ) 
-  {ψ} (h : ψ = sentence φ φ_h) (H: (sentence φ φ_h) ∈ Γ) : ψ ∈ Γ :=
+lemma mem {Γ:set $ fol.formula σ} (φ) (k) (φ_h: formula.closed (k+2) φ) 
+  {ψ} (h : ψ = separation.formula φ φ_h) (H: (separation.formula φ φ_h) ∈ Γ) : ψ ∈ Γ :=
 begin subst h, exact H, end 
 
-def scheme : set $ fol.formula 𝒮 := 
-  { (sentence φ φ_h) |  (φ : fol.formula 𝒮) (k: ℕ) (φ_h : formula.closed (k+2) φ) } 
+/-- Defintion of the axiom scheme of separation as set. -/
+def scheme : set $ fol.formula σ := 
+  { (separation.formula φ φ_h) |  (φ : fol.formula σ) (k: ℕ) (φ_h : formula.closed (k+2) φ) } 
 
-lemma mem_scheme (φ : fol.formula 𝒮) {k : ℕ} (φ_h: fol.formula.closed (k+2) φ)
-  : sentence φ φ_h ∈ scheme := begin existsi [φ, k, φ_h], refl end
+lemma mem_scheme (φ : fol.formula σ) {k : ℕ} (φ_h: fol.formula.closed (k+2) φ) : 
+  separation.formula φ φ_h ∈ scheme := begin existsi [φ, k, φ_h], refl end
  
 end separation
 
 
 namespace collection
-/-
-  The collection axiom scheme is defined as the closure of
-    `∀A ( ∀x(x ∈ A → ∃y φ) → ∃B ∀x (x ∈ A →  ∃y (y ∈ B ∧ φ)` (1)
-  for all formulas φ such that B is not free in φ.
-  Observe that in this case the the quantifier before B binds variables pointing to 2.
-  Thus the side condition can be stated as
-    `φ = ψ ↑ 1 ＠ 2` 
-  for a formula `ψ` and we obtain our axiom scheme as the closure of the formula below.
--/
-@[simp] def formula (φ: formula 𝒮) := 
-  (∀'( ∀'(#0 ∈' #1 →' ∃'φ) →' ( ∃' ∀' ( #0 ∈' #2 →' (∃' (#0 ∈' #2 ∧' (φ ↑ 1 ＠ 2))))))) 
-/-
-  To define the closure of (1) we usually state collection in terms of formulas φ(x, y, A, x₁, ... , xₙ)
-  with free variables among (but not necessarily exactly) x, y, A, x₁, ... , xₙ.
 
-  This then translates to `φ_h: closed (n+3) φ` and we can proceed as in the case of separation.
--/
-lemma closed  {φ} {k} (H: closed (k+3) φ) : closed k (formula φ) :=
+/-- Defintion of the axiom scheme of collection with free variables -/
+@[simp] def free_formula (φ: formula σ) := 
+  (∀'(∀'(#0 ∈' #1 →' ∃'φ) →' (∃' ∀' (#0 ∈' #2 →' (∃' (#0 ∈' #2 ∧' (φ ↑ 1 ＠ 2))))))) 
+
+lemma closed  {φ} {k} (H: formula.closed (k+3) φ) : formula.closed k (free_formula φ) :=
 begin
   have : ¬ k+4 ≤ 2, by linarith,
   have : ¬ k+3 ≤ 2, by linarith,
@@ -227,41 +192,34 @@ begin
   simp[*, closed],
 end 
 
-def sentence  (φ : fol.formula 𝒮) {k : ℕ} (H: formula.closed (k+3) φ) : fol.formula 𝒮 
-  := formula.closure (formula φ) (closed H)
+/-- Defintion of the axiom scheme of collection -/
+def formula (φ : fol.formula σ) {k : ℕ} (H: formula.closed (k+3) φ) : fol.formula σ 
+  := formula.closure (free_formula φ) (closed H)
 
-lemma is_sentence  (φ : fol.formula 𝒮) {k : ℕ} (H: fol.formula.closed (k+3) φ) :
-  (sentence φ H) is_sentence' := begin exact closure_is_sentence (closed H) end
+lemma formula_is_sentence  (φ : fol.formula σ) {k : ℕ} (H: fol.formula.closed (k+3) φ) :
+  (formula φ H) is_sentence := begin exact closure_is_sentence (closed H) end
 
 /- To following definition and lemmas are used to make future proofs more explicit and readable. -/
-lemma mem {Γ:set $ fol.formula 𝒮} {ψ} {k} (φ) (φ_h: formula.closed (k+3) φ) 
-  (h : ψ = sentence φ φ_h) (H: (sentence φ φ_h) ∈ Γ) : ψ ∈ Γ :=
+lemma mem {Γ:set $ fol.formula σ} {ψ} {k} (φ) (φ_h: formula.closed (k+3) φ) 
+  (h : ψ = formula φ φ_h) (H: (formula φ φ_h) ∈ Γ) : ψ ∈ Γ :=
 begin subst h, exact H end 
 
-def scheme : set $ fol.formula 𝒮 := 
-  { (sentence φ φ_h) |  (φ : fol.formula 𝒮) (k: ℕ) (φ_h : fol.formula.closed (k+3) φ) }
+/-- Defintion of the axiom scheme of collection as set -/
+def scheme : set $ fol.formula σ := 
+  { (formula φ φ_h) |  (φ : fol.formula σ) (k: ℕ) (φ_h : fol.formula.closed (k+3) φ) }
 
-lemma mem_scheme (φ : fol.formula 𝒮) {k : ℕ} (φ_h: fol.formula.closed (k+3) φ)
-  : sentence φ φ_h ∈ scheme := begin existsi [φ, k, φ_h], refl, end
+lemma mem_scheme (φ : fol.formula σ) {k : ℕ} (φ_h: fol.formula.closed (k+3) φ)
+  : formula φ φ_h ∈ scheme := begin existsi [φ, k, φ_h], refl, end
 
 end collection
 
+
 namespace set_induction
-/-
-  The set induction axiom scheme is defined as the closure of
-    `∀A (∀x (x ∈ A → φ(x)) → φ) → ∀A φ` (1)
-  for all formulas φ.
--/
-@[simp] def formula (φ: formula 𝒮) := 
-  (∀'(∀'(#0 ∈' #1 →' (φ ↑ 1 ＠ 1)) →' φ ) →' (∀'φ))
+/-- Defintion of the axiom scheme of set induction with free variables. -/ 
+@[simp] def free_formula (φ: formula σ) := 
+  (∀'(∀'(#0 ∈' #1 →' (φ ↑ 1 ＠ 1)) →' φ) →' (∀'φ))
 
-/-
-  To define the closure of (1) we usually state collection in terms of formulas φ( A, x₁, ... , xₙ)
-  with free variables among (but not necessarily exactly) A, x₁, ... , xₙ.
-
-  This then translates to `φ_h: closed (n+1) φ` and we can proceed as in the case of separation.
--/
-lemma closed  {φ} {n} (φ_h: closed (n+1) φ) : closed n (formula φ) :=
+lemma closed  {φ} {n} (φ_h: closed (n+1) φ) : closed n (free_formula φ) :=
 begin
   have : φ ↑ 1 ＠ 1 ↑ 1 ＠ (n + 1 + 1) = φ ↑ 1 ＠ 1 :=
   begin rw ←(lift_lift φ 1 1 (nat.succ_pos n)), congr, exact φ_h, end,
@@ -269,79 +227,78 @@ begin
   simp*,
 end 
 
-def sentence  (φ : fol.formula 𝒮) {n : ℕ} (φ_h: formula.closed (n+1) φ) : fol.formula 𝒮 
-  := formula.closure (formula φ) (closed φ_h)
+/-- Defintion of the axiom scheme of set induction -/
+def formula (φ : fol.formula σ) {n : ℕ} (φ_h: formula.closed (n+1) φ) : fol.formula σ 
+  := formula.closure (free_formula φ) (closed φ_h)
 
-lemma is_sentence  (φ : fol.formula 𝒮) {n : ℕ} (φ_h: fol.formula.closed (n+1) φ) :
-  (sentence φ φ_h) is_sentence' := begin exact closure_is_sentence (closed φ_h) end
+lemma formula_is_sentence (φ : fol.formula σ) {n : ℕ} (φ_h: fol.formula.closed (n+1) φ) :
+  (formula φ φ_h) is_sentence := begin exact closure_is_sentence (closed φ_h) end
 
 /- To following definition and lemmas are used to make future proofs more explicit and readable. -/
-lemma mem {Γ:set $ fol.formula 𝒮} {ψ} (φ) {n} (φ_h: formula.closed (n+1) φ) 
-  (h : ψ = sentence φ φ_h) (H: (sentence φ φ_h) ∈ Γ) : ψ ∈ Γ :=
+lemma mem {Γ:set $ fol.formula σ} {ψ} (φ) {n} (φ_h: formula.closed (n+1) φ) 
+  (h : ψ = formula φ φ_h) (H: (formula φ φ_h) ∈ Γ) : ψ ∈ Γ :=
 begin subst h, exact H end 
 
-def scheme : set $ fol.formula 𝒮 := 
-  { (sentence φ φ_h) |  (φ : fol.formula 𝒮) (k: ℕ) (φ_h : fol.formula.closed (k+1) φ) }
+/-- Defintion of the axiom scheme of set induction as set -/
+def scheme : set $ fol.formula σ := 
+  { (formula φ φ_h) |  (φ : fol.formula σ) (k: ℕ) (φ_h : fol.formula.closed (k+1) φ) }
 
-lemma mem_scheme (φ : fol.formula 𝒮) {k : ℕ} (φ_h: fol.formula.closed (k+1) φ)
-  : sentence φ φ_h ∈ scheme := begin existsi [φ, k, φ_h], refl, end
+lemma mem_scheme (φ : fol.formula σ) {k : ℕ} (φ_h: fol.formula.closed (k+1) φ)
+  : formula φ φ_h ∈ scheme := begin existsi [φ, k, φ_h], refl, end
 
 end set_induction
 
 
 /- ∀b ∀a (∀x (x ∈ a ↔ x ∈ b) → a = b) -/
-@[simp] def extensionality : formula 𝒮 := ∀' ∀' ( (∀' (#0 ∈' #1 ↔' #0 ∈' #2)) →' (#0 =' #1) )
-/- ∀x ( x ∈ ⌀ ↔ x ≠ x) -/
-@[simp] def emptyset_ax    : formula 𝒮 := ∀' (#0 ∈' ⌀ ↔' ¬'(#0 =' #0) )
+@[simp] def extensionality : formula σ := ∀' ∀' ((∀' (#0 ∈' #1 ↔' #0 ∈' #2)) →' (#0 =' #1))
+/- ∀x (x ∈ ⌀ ↔ x ≠ x) -/
+@[simp] def emptyset_ax    : formula σ := ∀' (#0 ∈' ⌀ ↔' ¬'(#0 =' #0))
 /- ∀b ∀a ∀x (x ∈{a,b} ↔ x = a ∨ x = b) -/
-@[simp] def pairset_ax     : formula 𝒮 := ∀' ∀' ∀' ( #0 ∈' ⦃ #1 , #2 ⦄ ↔' (#0 =' #1 ∨' #0 =' #2))
+@[simp] def pairset_ax     : formula σ := ∀' ∀' ∀' (#0 ∈' ⦃ #1 , #2 ⦄ ↔' (#0 =' #1 ∨' #0 =' #2))
 /- ∀F ∀x (x ∈ ⋃F ↔ ∃y (x ∈ y ∧ y ∈ x))  -/
-@[simp] def unionset_ax    : formula 𝒮 := ∀' ∀' ( #0 ∈' ⋃#1 ↔' ∃'( #1 ∈' #0 ∧' #0 ∈' #2))
+@[simp] def unionset_ax    : formula σ := ∀' ∀' (#0 ∈' ⋃#1 ↔' ∃'(#1 ∈' #0 ∧' #0 ∈' #2))
 /- ∀y ∀x (x ∈ 𝒫(y) → x ⊆ y) -/
-@[simp] def powerset_ax    : formula 𝒮 := ∀' ∀' (#0 ∈' 𝒫#1 ↔' #0 ⊆' #1)
-/- ∀x ( x ∈ ω ↔ ∀w (w is inductive → x ∈ w)) -/
-@[simp] def omega_ax       : formula 𝒮 := ∀' (#0 ∈' ω ↔' ∀'( (#0 is_inductive) →' #1 ∈' #0))
+@[simp] def powerset_ax    : formula σ := ∀' ∀' (#0 ∈' 𝒫#1 ↔' #0 ⊆' #1)
+/- ∀x (x ∈ ω ↔ ∀w (w is inductive → x ∈ w)) -/
+@[simp] def omega_ax       : formula σ := ∀' (#0 ∈' ω ↔' ∀'((#0 is_inductive) →' #1 ∈' #0))
 /- ∀xₙ ... ∀x₁ ∀A (∀x (x ∈ A → φ(x)) → φ(A)) → ∀A φ(A) -/
-@[simp] def set_induction_ax  (φ : formula 𝒮) {n : ℕ} (φ_h: closed (n+1) φ) : formula 𝒮  
-  := set_induction.sentence φ φ_h
-/-- ∀xₙ ... ∀x₁ ∀A ∃B ∀x ( x ∈ B ↔ x ∈ A ∧ φ ↑ 1 ＠ 1) -/
-@[simp] def separation_ax  (φ : formula 𝒮) {n: ℕ} (φ_h: closed (n+2) φ) : formula 𝒮 
-  := separation.sentence φ φ_h
-/-- ∀xₙ ... ∀x₁ ∀A ( ∀x(x ∈ A → ∃y φ) → ∃B ∀x (x ∈ A →  ∃y (y ∈ B ∧ φ) -/
-@[simp] def collection_ax (φ : formula 𝒮) {n : ℕ} (φ_h: closed (n+3) φ) : formula 𝒮 
-  := collection.sentence φ φ_h
+@[simp] def set_induction_ax  (φ : formula σ) {n : ℕ} (φ_h: closed (n+1) φ) : formula σ  
+  := set_induction.formula φ φ_h
+/-- ∀xₙ ... ∀x₁ ∀A ∃B ∀x (x ∈ B ↔ x ∈ A ∧ φ ↑ 1 ＠ 1) -/
+@[simp] def separation_ax  (φ : formula σ) {n: ℕ} (φ_h: closed (n+2) φ) : formula σ 
+  := separation.formula φ φ_h
+/-- ∀xₙ ... ∀x₁ ∀A (∀x(x ∈ A → ∃y φ) → ∃B ∀x (x ∈ A →  ∃y (y ∈ B ∧ φ) -/
+@[simp] def collection_ax (φ : formula σ) {n : ℕ} (φ_h: closed (n+3) φ) : formula σ 
+  := collection.formula φ φ_h
 
 -- optional: definition of the subset predicate
--- @[simp] def subset_def   : formula 𝒮 := ∀' ∀' ( #0 ⊆' #1  ↔' ∀' (#0 ∈' #1 →' #0 ∈' #2) )
+-- @[simp] def subset_def   : formula σ := ∀' ∀' (#0 ⊆' #1  ↔' ∀' (#0 ∈' #1 →' #0 ∈' #2))
 
 /-
- * The following lemmas provide a convenient way to make explicit which axioms are used inside our proofs.
- * For separation and collection we can use separation.mem and collection.mem respectively.
+ The following lemmas provide a convenient way to make explicit which axioms are used inside our proofs.
 -/
-lemma extensionality_mem {Γ: set $ formula 𝒮}{φ}(h: φ = extensionality)(H: extensionality ∈ Γ) : φ ∈ Γ :=
+lemma extensionality_mem {Γ: set $ formula σ}{φ}(h: φ = extensionality)(H: extensionality ∈ Γ) : φ ∈ Γ :=
 begin subst h, exact H end
-lemma emptyset_ax_mem {Γ: set $ formula 𝒮} {φ} (h: φ = emptyset_ax) (H: emptyset_ax ∈ Γ)  : φ ∈ Γ :=
+lemma emptyset_ax_mem {Γ: set $ formula σ} {φ} (h: φ = emptyset_ax) (H: emptyset_ax ∈ Γ)  : φ ∈ Γ :=
 begin subst h, exact H end
-lemma pairset_ax_mem {Γ: set $ formula 𝒮} {φ} (h: φ = pairset_ax) (H: pairset_ax ∈ Γ)  : φ ∈ Γ :=
+lemma pairset_ax_mem {Γ: set $ formula σ} {φ} (h: φ = pairset_ax) (H: pairset_ax ∈ Γ)  : φ ∈ Γ :=
 begin subst h, exact H end
-lemma unionset_ax_mem {Γ: set $ formula 𝒮} {φ} (h: φ = unionset_ax) (H: unionset_ax ∈ Γ)  : φ ∈ Γ :=
+lemma unionset_ax_mem {Γ: set $ formula σ} {φ} (h: φ = unionset_ax) (H: unionset_ax ∈ Γ)  : φ ∈ Γ :=
 begin subst h, exact H end
-lemma powerset_ax_mem {Γ: set $ formula 𝒮} {φ} (H: powerset_ax ∈ Γ) (h: φ = powerset_ax) : φ ∈ Γ :=
+lemma powerset_ax_mem {Γ: set $ formula σ} {φ} (H: powerset_ax ∈ Γ) (h: φ = powerset_ax) : φ ∈ Γ :=
 begin subst h, exact H end
-lemma omega_ax_mem {Γ: set $ formula 𝒮} {φ} (h: φ = omega_ax) (H: omega_ax ∈ Γ) : φ ∈ Γ :=
+lemma omega_ax_mem {Γ: set $ formula σ} {φ} (h: φ = omega_ax) (H: omega_ax ∈ Γ) : φ ∈ Γ :=
 begin subst h, exact H end
 
 
-/--
-  The set of axioms for IZF.
--/
-def izf_ax : set $ formula 𝒮 := { extensionality, emptyset_ax, pairset_ax, 
+/-- The set of axioms for IZF. -/
+def izf_ax : set $ formula σ := { extensionality, emptyset_ax, pairset_ax, 
                                   unionset_ax, powerset_ax, omega_ax } 
                                   ∪ set_induction.scheme
                                   ∪ separation.scheme
                                   ∪ collection.scheme
 
-lemma izf_ax_set_of_sentences : ∀ ϕ ∈ izf_ax , sentence ϕ :=
+lemma izf_ax_set_of_sentences : ∀ φ ∈ izf_ax, φ is_sentence :=
 begin
   intros φ h,
   repeat {cases h,};
@@ -349,12 +306,12 @@ begin
   all_goals { cases h_h with k H,
               cases H with ϕ_closed,
               subst H_h },
-  exact set_induction.is_sentence _ ϕ_closed,
-  exact separation.is_sentence _ ϕ_closed,
-  exact collection.is_sentence _ ϕ_closed,
+  exact set_induction.formula_is_sentence _ ϕ_closed,
+  exact separation.formula_is_sentence _ ϕ_closed,
+  exact collection.formula_is_sentence _ ϕ_closed,
 end
 
-lemma lift_izf_ax {m i : ℕ}: (λ (ϕ: formula 𝒮) , ϕ ↑ m ＠ i) '' izf_ax = izf_ax 
+lemma lift_izf_ax {m i : ℕ}: (λ (ϕ: formula σ) , ϕ ↑ m ＠ i) '' izf_ax = izf_ax 
   := lift_set_of_sentences_id izf_ax_set_of_sentences
 
 end izf_axioms
@@ -365,21 +322,21 @@ section izf_proofs
 /--
   Proof scheme. 
   Provides a formal proof of uniqueness of y
-  satisfying formulas of the form `∀x (x ∈ y ↔ φ )`,
+  satisfying formulas of the form `∀x (x ∈ y ↔ φ)`,
   provided `y` is not free in `φ`.
 
-  Informally : {extensionality} ⊢ ∀y₁ ∀y₀ ( y₀ = { x | φ } ∧ y₁ = { x | φ } → y₀ = y₁)
+  Informally : {extensionality} ⊢ ∀y₁ ∀y₀ (y₀ = { x | φ } ∧ y₁ = { x | φ } → y₀ = y₁)
 -/
-def extensionality_implies_uniqueness (φ : formula 𝒮)
+def extensionality_implies_uniqueness (φ : formula σ)
   : {extensionality} ⊢ unique_in_var0  ∀'(#0 ∈' #1 ↔' (φ ↑ 1 ＠ 1)) :=
 begin
   apply allI, -- y₁
   apply allI, -- y₀
-  apply impI, -- assume `∀ x ( x ∈ y₀ ↔ φ(x, y₀)) ∧ ∀ x (x ∈ y₁ ↔ φ(x,y₁))`
+  apply impI, -- assume `∀ x (x ∈ y₀ ↔ φ(x, y₀)) ∧ ∀ x (x ∈ y₁ ↔ φ(x,y₁))`
   apply impE (∀' (#0 ∈' #1 ↔' #0 ∈' #2)), 
   { -- y₁ y₀ ⊢ (∀' (#0 ∈' #1 ↔' #0 ∈' #2))
     apply allI, -- x
-    apply iffI_trans (φ ↑ 2 ＠  1), 
+    apply iffI_trans (φ ↑ 2 ＠ 1), 
     { -- y₁ y₀ x ⊢ x ∈ y₀ ↔ φ (x, y₀)
       apply allE_var0, 
       apply andE₁ _ , 
@@ -408,9 +365,9 @@ end
   QoL version of `extensionality_implies_uniqueness`
 
   Informally : `Γ ⊢ ∀y₁ ∀y₀ (ψ(y₀) ∧ ψ(y₁) → y₀ = y₁`,
-  provided  `ψ(y) = ∀x (x ∈ y ↔ φ )`, `y` not free in `φ` and `extensionality ∈ Γ`.
+  provided  `ψ(y) = ∀x (x ∈ y ↔ φ)`, `y` not free in `φ` and `extensionality ∈ Γ`.
 -/
-def extensionality_implies_uniqueness' {Γ} (φ) {ψ} (h: ψ = ∀'(#0 ∈' #1 ↔' (φ ↑ 1 ＠ 1) ) ) (H: extensionality ∈ Γ)  
+def extensionality_implies_uniqueness' {Γ} (φ) {ψ} (h: ψ = ∀'(#0 ∈' #1 ↔' (φ ↑ 1 ＠ 1))) (H: extensionality ∈ Γ)  
   : Γ ⊢ unique_in_var0 ψ :=
 begin
   subst h,
@@ -421,9 +378,9 @@ end
 /--
   `n`-closure variant of `extensionality_implies_uniqueness` 
 
-  Informally : `{extensionality} ⊢ ∀xₙ ... ∀x₁ ∀y₁ ∀y₀ ( y₀ = { x | φ } ∧ y₁ = { x | φ } → y₀ = y₁)`
+  Informally : `{extensionality} ⊢ ∀xₙ ... ∀x₁ ∀y₁ ∀y₀ (y₀ = { x | φ } ∧ y₁ = { x | φ } → y₀ = y₁)`
 -/
-def extensionality_implies_uniqueness_alls  (n)  (φ : formula 𝒮)
+def extensionality_implies_uniqueness_alls  (n)  (φ : formula σ)
   : {extensionality} ⊢ alls n (unique_in_var0 ∀'(#0 ∈' #1 ↔' (φ ↑ 1 ＠ 1))) :=
 begin
   apply allsI,
@@ -434,24 +391,24 @@ begin
 end
 
 /--
-  Proof scheme. Provides a formal oroof of `∃B ∀x(x ∈ B ↔ φ)`
-  from `∃B ∀x ( φ → x ∈ B)` by using the axiom of separation for `φ`.
+  Proof scheme. Provides a formal proof of `∃B ∀x(x ∈ B ↔ φ)`
+  from `∃B ∀x (φ → x ∈ B)` by using the axiom of separation for `φ`.
 -/
 def separation_proof_scheme 
   (φ k) (φ_h₁: closed (k+2) φ)              -- given a formula φ(x_1,...,x_{k+1})
-  (φ_h₂ : ∃ ϕ : formula 𝒮 , φ = ϕ ↑ 1 ＠ 1) -- such that the x₂ is not among its free variables
+  (φ_h₂ : not_free 1 φ) -- such that the x₂ is not among its free variables
   {Γ} (h : separation_ax φ φ_h₁ ∈ Γ)        -- ...
   (H : Γ ⊢ alls k ∃' ∀'(φ →' (#0 ∈' #1)))
   : Γ ⊢ alls k (∃' ∀'((#0 ∈' #1) ↔' φ)) :=
 begin
   apply allsI,
-  apply exE ∀'( φ →' (#0 ∈' #1)), -- A with ∀ x (φ → x ∈ A) 
+  apply exE ∀'(φ →' (#0 ∈' #1)), -- A with ∀ x (φ → x ∈ A) 
   { -- xₖ ... x₁ ⊢ ∃ A ∀x (φ → x ∈ A)
     apply allsE',
     exact H },
-  { -- xₖ ... x₁ A ⊢ ∃ B ∀ x (x ∈ B ↔ φ )
-    apply exE (∀'( (#0 ∈' #1) ↔' ( (#0 ∈' #2) ∧' (φ ↑ 1 ＠ 1 ) ))), -- B with ∀ x (x ∈ B ↔ x ∈ A ∧ φ )
-    { -- xₖ ... x₁ A ⊢ ∃ B ∀ x (x ∈ B ↔ x ∈ A ∧ φ )
+  { -- xₖ ... x₁ A ⊢ ∃ B ∀ x (x ∈ B ↔ φ)
+    apply exE (∀'((#0 ∈' #1) ↔' ((#0 ∈' #2) ∧' (φ ↑ 1 ＠ 1)))), -- B with ∀ x (x ∈ B ↔ x ∈ A ∧ φ)
+    { -- xₖ ... x₁ A ⊢ ∃ B ∀ x (x ∈ B ↔ x ∈ A ∧ φ)
       apply weak1, 
       apply allsE' 1,
       apply allsE' k,
@@ -460,7 +417,7 @@ begin
       -- meta
       apply separation.mem φ k φ_h₁ (rfl),
       assumption, },
-    { -- A B ⊢ ∃ B ∀ x (x ∈ B ↔ φ ) 
+    { -- A B ⊢ ∃ B ∀ x (x ∈ B ↔ φ) 
       apply exI #0,
       apply allI, -- x
       apply andI,
@@ -525,12 +482,12 @@ end
   QoL version of `separation_proof_scheme`.
   
   Proof scheme. Provides a formal proof `ψ`
-  from `∃B ∀x ( φ → x ∈ B)` and `ψ = ∃B ∀x(x ∈ B ↔ φ)`.
+  from `∃B ∀x (φ → x ∈ B)` and `ψ = ∃B ∀x(x ∈ B ↔ φ)`.
 -/
 def separation_proof_scheme' (φ) (k) (φ_h: closed (k+2) (φ ↑ 1 ＠ 1))
-  {ψ : formula 𝒮} (ψ_h : ψ = alls k ∃' ∀'((#0 ∈' #1) ↔' (φ  ↑ 1 ＠ 1)))
-  {Γ} (h : separation.sentence (φ ↑ 1 ＠ 1) φ_h ∈ Γ)
-  (H: Γ ⊢ alls k ∃' ∀'( φ  ↑ 1 ＠ 1  →' (#0 ∈' #1))) 
+  {ψ : formula σ} (ψ_h : ψ = alls k ∃' ∀'((#0 ∈' #1) ↔' (φ ↑ 1 ＠ 1)))
+  {Γ} (h : separation.formula (φ ↑ 1 ＠ 1) φ_h ∈ Γ)
+  (H: Γ ⊢ alls k ∃' ∀'(φ ↑ 1 ＠ 1  →' (#0 ∈' #1))) 
   : Γ ⊢ ψ  :=
 begin
   subst ψ_h,
@@ -574,7 +531,7 @@ begin
     { -- a x ⊢ x = a ∨ x = a 
       apply orI₁, 
       apply hypI1, },
-    { -- a x ⊢ (x = a ∨ x = a ) → x ∈ {a}
+    { -- a x ⊢ (x = a ∨ x = a) → x ∈ {a}
       apply iffE_l, 
       apply allE_var0,
       apply allE' _ #1,
@@ -589,7 +546,7 @@ end
   Informally: `Γ ⊢ φ` provided `φ = ∀ a : { a } = { x | x = a }`
   and `pairset_ax ∈ Γ`.
 -/
-def singleton_def' {Γ} {φ : formula 𝒮} (h₁: φ = ∀' ∀' (#0 ∈' ⦃ #1 ⦄ ↔' #0 =' #1)) (h₂ : pairset_ax ∈ Γ ) :
+def singleton_def' {Γ} {φ : formula σ} (h₁: φ = ∀' ∀' (#0 ∈' ⦃ #1 ⦄ ↔' #0 =' #1)) (h₂ : pairset_ax ∈ Γ) :
   Γ ⊢ φ  :=
 begin
   subst h₁,
@@ -626,7 +583,7 @@ begin
     { -- b a x y ⊢ x ∈ a ∨ x ∈ b
       apply impE (#0 =' #2 ∨' #0 =' #3),
       { -- b a x y ⊢ y = a ∨ y = b
-        apply impE (#0 ∈'  ⦃#2 , #3⦄ ),
+        apply impE (#0 ∈'  ⦃#2 , #3⦄),
         { -- b a x y ⊢ y ∈ {a,b}
           apply andE₂, 
           apply hypI1 },
@@ -694,7 +651,7 @@ begin
             apply pairset_ax_mem (rfl),
             all_goals { try { simp[set.image_insert_eq], }, },
             split; refl } } },
-      { -- b a x ⊢ ∃y ( x ∈ y ∧ y ∈ {a,b}) → x ∈ a ∪ b
+      { -- b a x ⊢ ∃y (x ∈ y ∧ y ∈ {a,b}) → x ∈ a ∪ b
         apply iffE_l ,
         apply allE_var0,
         apply allE' _ ⦃ #1 , #2 ⦄,
@@ -724,7 +681,7 @@ begin
             apply pairset_ax_mem (rfl),
             all_goals { try { simp[set.image_insert_eq], }, },
             split; refl } } },
-      { -- b a x ⊢ ∃y ( x ∈ y ∧ y ∈ {a,b}) → x ∈ a ∪ b
+      { -- b a x ⊢ ∃y (x ∈ y ∧ y ∈ {a,b}) → x ∈ a ∪ b
         apply iffE_l ,
         apply allE_var0,
         apply allE' _ ⦃ #1 , #2 ⦄,
@@ -738,8 +695,8 @@ end
   Informally: `Γ ⊢ φ` provided `φ =  ∀ b ∀ a : a ∪ b = { x | x ∈ a ∨ x ∈ b }`
   and `pairset_ax, unionset_ax ∈ Γ`.
 -/
-def binary_union_def' {Γ} {φ : formula 𝒮} (h₁: φ = ∀' ∀' ∀'(#0 ∈' ⋃ ⦃ #1, #2 ⦄ ↔' #0 ∈' #1 ∨' #0 ∈' #2) )
-  (h₂: pairset_ax ∈ Γ ) (h₃ : unionset_ax ∈ Γ) : Γ  ⊢ φ :=
+def binary_union_def' {Γ} {φ : formula σ} (h₁: φ = ∀' ∀' ∀'(#0 ∈' ⋃ ⦃ #1, #2 ⦄ ↔' #0 ∈' #1 ∨' #0 ∈' #2))
+  (h₂: pairset_ax ∈ Γ) (h₃ : unionset_ax ∈ Γ) : Γ  ⊢ φ :=
 begin
   subst h₁,
   apply weak {pairset_ax, unionset_ax},
@@ -780,7 +737,7 @@ begin
         all_goals{ simp[set.image_insert_eq] } } },
     { -- a x ⊢ x ∈ a ∨ x ∈ {a} → x ∈ a ∨ x = a
       apply impI, -- assume `x ∈ a ∨ x ∈ {a}`
-      apply orE (#0 ∈' #1) ( #0 ∈' ⦃ #1 ⦄),
+      apply orE (#0 ∈' #1) (#0 ∈' ⦃ #1 ⦄),
       { -- a x ⊢ x ∈ a ∨ x ∈ {a}
         apply hypI1, },
       { -- assume `x ∈ a`
@@ -835,25 +792,24 @@ begin
 end
 
 
-/--
-  Formal proof that there (trivially) exists a set 
-  containing exactly the elements common to all inductive sets
-  and that such a set is unique,
-  derived from the omega axiom and extensionality.
-
-  Informally: `{omega_ax, extensionality} ⊢ ∃! w₀ : w₀ = { x | ∀ w : (w is inductive) →  x ∈ w }`.
--/
+/-- Formal proof that ω is unique. -/
 def omega_unique 
-  : {omega_ax, extensionality} ⊢ ∃! ∀' (#0 ∈' #1 ↔' ∀'( (#0 is_inductive) →' #1 ∈' #0)) := 
+  : ∅ ⊢ ∃! (#0 =' ω) := 
 begin
   apply andI,
   { -- ∃ case is trivial
     apply exI ω,
-    apply hypI,
-    simp },
+    apply eqI },
   { -- uniqueness
-    apply extensionality_implies_uniqueness' (∀'(#0 is_inductive →' #1 ∈' #0)) (rfl),
-    simp }
+    apply allsI 2,
+    apply impI,
+    apply eqE' ω #1 (#1 =' #0),
+    { apply eqI_symm,
+      apply andE₂,
+      apply hypI1, },
+    { apply andE₁,
+      apply hypI1,},
+    { refl, }, },
 end
 
 /--
@@ -905,23 +861,23 @@ begin
   apply andI,
   { -- ⊢ ⌀ ∈ ω
     apply impE ∀'(#0 is_inductive →' ⌀ ∈' #0), 
-    { -- ⊢ ∀ w ( w is inductive → ⌀ ∈ w)
+    { -- ⊢ ∀ w (w is inductive → ⌀ ∈ w)
       apply allI,
       apply impI,
       apply andE₁,
       apply hypI,
       simp },
-    { -- ⊢ ∀ w ( w is inductive → ⌀ ∈ w) → ⌀ ∈ ω
+    { -- ⊢ ∀ w (w is inductive → ⌀ ∈ w) → ⌀ ∈ ω
       apply iffE_l,
       apply allE' _ ⌀,
       apply hypI,
       apply omega_ax_mem (rfl),
       all_goals { simp } } },
-  { -- ⊢ ∀ x ( x ∈ ω → S(x) ∈ ω)
+  { -- ⊢ ∀ x (x ∈ ω → S(x) ∈ ω)
     apply allI, -- x
     apply impI, -- assume `x ∈ ω`
     apply impE (∀'(#0 is_inductive →' S#1 ∈' #0)),
-    { -- x  ⊢ ∀ w ( (w is inductive) → S(x) ∈ w)
+    { -- x  ⊢ ∀ w ((w is inductive) → S(x) ∈ w)
       apply allI, -- w
       apply impI, -- assume `w is inductive`
       apply impE (#1 ∈' #0),
@@ -941,7 +897,7 @@ begin
         apply allE' (#0 ∈' #1 →' S #0 ∈' #1) #1 _ (rfl),
         apply andE₂ _ ,
         apply hypI1 } },
-    { -- x ⊢ ∀ w ( (w is inductive) → S(x) ∈ w) → S(x) ∈ ω
+    { -- x ⊢ ∀ w ((w is inductive) → S(x) ∈ w) → S(x) ∈ ω
       apply iffE_l,
       apply allE' _ S#0,
       apply hypI,
@@ -964,18 +920,20 @@ end
 
   Informally : `izf_ax ⊢ (ω is inductive) ∧ ∀ w ((w is inductive) → ω ⊆ w)`
 -/
-def omega_smallest_inductive : izf_ax ⊢ (ω is_inductive) ∧' ∀'((#0 is_inductive) →' ω ⊆' #0) :=
+def omega_smallest_inductive : izf_ax ⊢ 
+  (ω is_inductive) ∧' ∀'((#0 is_inductive) →' ω ⊆' #0) :=
 begin
   apply andI,
-  { apply omega_inductive', simp[izf_ax], },
-  { apply omega_subset_all_inductive', simp[izf_ax], },
+  { apply omega_inductive', simp[izf_ax] },
+  { apply omega_subset_all_inductive', simp[izf_ax], } 
 end
 
 end izf_proofs
 
 /--  Main Theorem: IZF proves that ω is the smallest inductive set. -/
-theorem omega_smallest_inductive_provable_within_izf : 
-  ((ω is_inductive) ∧' ∀'((#0 is_inductive) →' ω ⊆' #0)) is_provable_within izf_ax :=
+theorem omega_smallest_inductive_provable: 
+  ((ω is_inductive) ∧' ∀'((#0 is_inductive) →' ω ⊆' #0))
+  is_provable_within izf_ax :=
 begin use omega_smallest_inductive end
 
 end izf 
