src/tls_tactic.lean
@@ -1,0 +1,12 @@
+open tactic interactive interactive.types
+
+namespace tactic
+namespace interactive
+
+/- apply followed by simp with tls. not yet useful -/
+meta def sapply (q : parse texpr) : tactic unit :=
+  concat_tags (do h ← i_to_expr_for_apply q, tactic.apply h) 
+  >> (simp none none ff {} {"tls"} (loc.ns [none]) )
+
+end interactive
+end tactic
